tuned whitespace;

src/Doc/Isar_Ref/Inner_Syntax.thy
@@ -6,26 +6,25 @@ begin
 
 chapter \<open>Inner syntax --- the term language \label{ch:inner-syntax}\<close>
 
-text \<open>The inner syntax of Isabelle provides concrete notation for
-  the main entities of the logical framework, notably \<open>\<lambda>\<close>-terms with types and type classes.  Applications may either
-  extend existing syntactic categories by additional notation, or
-  define new sub-languages that are linked to the standard term
-  language via some explicit markers.  For example \<^verbatim>\<open>FOO\<close>~\<open>foo\<close> could
-  embed the syntax corresponding for some
-  user-defined nonterminal \<open>foo\<close> --- within the bounds of the
-  given lexical syntax of Isabelle/Pure.
+text \<open>
+  The inner syntax of Isabelle provides concrete notation for the main
+  entities of the logical framework, notably \<open>\<lambda>\<close>-terms with types and type
+  classes. Applications may either extend existing syntactic categories by
+  additional notation, or define new sub-languages that are linked to the
+  standard term language via some explicit markers. For example \<^verbatim>\<open>FOO\<close>~\<open>foo\<close>
+  could embed the syntax corresponding for some user-defined nonterminal \<open>foo\<close>
+  --- within the bounds of the given lexical syntax of Isabelle/Pure.
 
-  The most basic way to specify concrete syntax for logical entities
-  works via mixfix annotations (\secref{sec:mixfix}), which may be
-  usually given as part of the original declaration or via explicit
-  notation commands later on (\secref{sec:notation}).  This already
-  covers many needs of concrete syntax without having to understand
-  the full complexity of inner syntax layers.
+  The most basic way to specify concrete syntax for logical entities works via
+  mixfix annotations (\secref{sec:mixfix}), which may be usually given as part
+  of the original declaration or via explicit notation commands later on
+  (\secref{sec:notation}). This already covers many needs of concrete syntax
+  without having to understand the full complexity of inner syntax layers.
 
-  Further details of the syntax engine involves the classical
-  distinction of lexical language versus context-free grammar (see
-  \secref{sec:pure-syntax}), and various mechanisms for \<^emph>\<open>syntax
-  transformations\<close> (see \secref{sec:syntax-transformations}).
+  Further details of the syntax engine involves the classical distinction of
+  lexical language versus context-free grammar (see \secref{sec:pure-syntax}),
+  and various mechanisms for \<^emph>\<open>syntax transformations\<close> (see
+  \secref{sec:syntax-transformations}).
 \<close>
 
 
@@ -63,43 +62,39 @@ text \<open>
     @{syntax_def modes}: '(' (@{syntax name} + ) ')'
   \<close>}
 
-  \<^descr> @{command "typ"}~\<open>\<tau>\<close> reads and prints a type expression
-  according to the current context.
+  \<^descr> @{command "typ"}~\<open>\<tau>\<close> reads and prints a type expression according to the
+  current context.
 
-  \<^descr> @{command "typ"}~\<open>\<tau> :: s\<close> uses type-inference to
-  determine the most general way to make \<open>\<tau>\<close> conform to sort
-  \<open>s\<close>.  For concrete \<open>\<tau>\<close> this checks if the type
-  belongs to that sort.  Dummy type parameters ``\<open>_\<close>''
-  (underscore) are assigned to fresh type variables with most general
-  sorts, according the the principles of type-inference.
+  \<^descr> @{command "typ"}~\<open>\<tau> :: s\<close> uses type-inference to determine the most
+  general way to make \<open>\<tau>\<close> conform to sort \<open>s\<close>. For concrete \<open>\<tau>\<close> this checks if
+  the type belongs to that sort. Dummy type parameters ``\<open>_\<close>'' (underscore)
+  are assigned to fresh type variables with most general sorts, according the
+  the principles of type-inference.
 
-  \<^descr> @{command "term"}~\<open>t\<close> and @{command "prop"}~\<open>\<phi>\<close>
-  read, type-check and print terms or propositions according to the
-  current theory or proof context; the inferred type of \<open>t\<close> is
-  output as well.  Note that these commands are also useful in
-  inspecting the current environment of term abbreviations.
+    \<^descr> @{command "term"}~\<open>t\<close> and @{command "prop"}~\<open>\<phi>\<close> read, type-check and
+    print terms or propositions according to the current theory or proof
+    context; the inferred type of \<open>t\<close> is output as well. Note that these
+    commands are also useful in inspecting the current environment of term
+    abbreviations.
 
-  \<^descr> @{command "thm"}~\<open>a\<^sub>1 \<dots> a\<^sub>n\<close> retrieves
-  theorems from the current theory or proof context.  Note that any
-  attributes included in the theorem specifications are applied to a
-  temporary context derived from the current theory or proof; the
-  result is discarded, i.e.\ attributes involved in \<open>a\<^sub>1,
-  \<dots>, a\<^sub>n\<close> do not have any permanent effect.
+    \<^descr> @{command "thm"}~\<open>a\<^sub>1 \<dots> a\<^sub>n\<close> retrieves theorems from the current theory
+    or proof context. Note that any attributes included in the theorem
+    specifications are applied to a temporary context derived from the current
+    theory or proof; the result is discarded, i.e.\ attributes involved in
+    \<open>a\<^sub>1, \<dots>, a\<^sub>n\<close> do not have any permanent effect.
 
-  \<^descr> @{command "prf"} displays the (compact) proof term of the
-  current proof state (if present), or of the given theorems. Note
-  that this requires proof terms to be switched on for the current
-  object logic (see the ``Proof terms'' section of the Isabelle
-  reference manual for information on how to do this).
+    \<^descr> @{command "prf"} displays the (compact) proof term of the current proof
+    state (if present), or of the given theorems. Note that this requires
+    proof terms to be switched on for the current object logic (see the
+    ``Proof terms'' section of the Isabelle reference manual for information
+    on how to do this).
 
-  \<^descr> @{command "full_prf"} is like @{command "prf"}, but displays
-  the full proof term, i.e.\ also displays information omitted in the
-  compact proof term, which is denoted by ``\<open>_\<close>'' placeholders
-  there.
+    \<^descr> @{command "full_prf"} is like @{command "prf"}, but displays the full
+    proof term, i.e.\ also displays information omitted in the compact proof
+    term, which is denoted by ``\<open>_\<close>'' placeholders there.
 
-  \<^descr> @{command "print_state"} prints the current proof state (if
-  present), including current facts and goals.
-
+    \<^descr> @{command "print_state"} prints the current proof state (if present),
+    including current facts and goals.
 
   All of the diagnostic commands above admit a list of \<open>modes\<close> to be
   specified, which is appended to the current print mode; see also
@@ -109,9 +104,8 @@ text \<open>
   symbols and special characters represented in {\LaTeX} source, according to
   the Isabelle style @{cite "isabelle-system"}.
 
-  Note that antiquotations (cf.\ \secref{sec:antiq}) provide a more
-  systematic way to include formal items into the printed text
-  document.
+  Note that antiquotations (cf.\ \secref{sec:antiq}) provide a more systematic
+  way to include formal items into the printed text document.
 \<close>
 
 
@@ -137,100 +131,90 @@ text \<open>
   \end{tabular}
   \<^medskip>
 
-  These configuration options control the detail of information that
-  is displayed for types, terms, theorems, goals etc.  See also
+  These configuration options control the detail of information that is
+  displayed for types, terms, theorems, goals etc. See also
   \secref{sec:config}.
 
-  \<^descr> @{attribute show_markup} controls direct inlining of markup
-  into the printed representation of formal entities --- notably type
-  and sort constraints.  This enables Prover IDE users to retrieve
-  that information via tooltips or popups while hovering with the
-  mouse over the output window, for example.  Consequently, this
-  option is enabled by default for Isabelle/jEdit.
+  \<^descr> @{attribute show_markup} controls direct inlining of markup into the
+  printed representation of formal entities --- notably type and sort
+  constraints. This enables Prover IDE users to retrieve that information via
+  tooltips or popups while hovering with the mouse over the output window, for
+  example. Consequently, this option is enabled by default for Isabelle/jEdit.
 
-  \<^descr> @{attribute show_types} and @{attribute show_sorts} control
-  printing of type constraints for term variables, and sort
-  constraints for type variables.  By default, neither of these are
-  shown in output.  If @{attribute show_sorts} is enabled, types are
-  always shown as well.  In Isabelle/jEdit, manual setting of these
-  options is normally not required thanks to @{attribute show_markup}
-  above.
+  \<^descr> @{attribute show_types} and @{attribute show_sorts} control printing of
+  type constraints for term variables, and sort constraints for type
+  variables. By default, neither of these are shown in output. If @{attribute
+  show_sorts} is enabled, types are always shown as well. In Isabelle/jEdit,
+  manual setting of these options is normally not required thanks to
+  @{attribute show_markup} above.
 
-  Note that displaying types and sorts may explain why a polymorphic
-  inference rule fails to resolve with some goal, or why a rewrite
-  rule does not apply as expected.
+  Note that displaying types and sorts may explain why a polymorphic inference
+  rule fails to resolve with some goal, or why a rewrite rule does not apply
+  as expected.
 
-  \<^descr> @{attribute show_consts} controls printing of types of
-  constants when displaying a goal state.
+  \<^descr> @{attribute show_consts} controls printing of types of constants when
+  displaying a goal state.
 
-  Note that the output can be enormous, because polymorphic constants
-  often occur at several different type instances.
+  Note that the output can be enormous, because polymorphic constants often
+  occur at several different type instances.
 
-  \<^descr> @{attribute show_abbrevs} controls folding of constant
-  abbreviations.
+  \<^descr> @{attribute show_abbrevs} controls folding of constant abbreviations.
 
-  \<^descr> @{attribute show_brackets} controls bracketing in pretty
-  printed output.  If enabled, all sub-expressions of the pretty
-  printing tree will be parenthesized, even if this produces malformed
-  term syntax!  This crude way of showing the internal structure of
-  pretty printed entities may occasionally help to diagnose problems
-  with operator priorities, for example.
+  \<^descr> @{attribute show_brackets} controls bracketing in pretty printed output.
+  If enabled, all sub-expressions of the pretty printing tree will be
+  parenthesized, even if this produces malformed term syntax! This crude way
+  of showing the internal structure of pretty printed entities may
+  occasionally help to diagnose problems with operator priorities, for
+  example.
 
-  \<^descr> @{attribute names_long}, @{attribute names_short}, and
-  @{attribute names_unique} control the way of printing fully
-  qualified internal names in external form.  See also
-  \secref{sec:antiq} for the document antiquotation options of the
-  same names.
+  \<^descr> @{attribute names_long}, @{attribute names_short}, and @{attribute
+  names_unique} control the way of printing fully qualified internal names in
+  external form. See also \secref{sec:antiq} for the document antiquotation
+  options of the same names.
 
-  \<^descr> @{attribute eta_contract} controls \<open>\<eta>\<close>-contracted
-  printing of terms.
+  \<^descr> @{attribute eta_contract} controls \<open>\<eta>\<close>-contracted printing of terms.
 
-  The \<open>\<eta>\<close>-contraction law asserts @{prop "(\<lambda>x. f x) \<equiv> f"},
-  provided \<open>x\<close> is not free in \<open>f\<close>.  It asserts
-  \<^emph>\<open>extensionality\<close> of functions: @{prop "f \<equiv> g"} if @{prop "f x \<equiv>
-  g x"} for all \<open>x\<close>.  Higher-order unification frequently puts
-  terms into a fully \<open>\<eta>\<close>-expanded form.  For example, if \<open>F\<close> has type \<open>(\<tau> \<Rightarrow> \<tau>) \<Rightarrow> \<tau>\<close> then its expanded form is @{term
-  "\<lambda>h. F (\<lambda>x. h x)"}.
+  The \<open>\<eta>\<close>-contraction law asserts @{prop "(\<lambda>x. f x) \<equiv> f"}, provided \<open>x\<close> is not
+  free in \<open>f\<close>. It asserts \<^emph>\<open>extensionality\<close> of functions: @{prop "f \<equiv> g"} if
+  @{prop "f x \<equiv> g x"} for all \<open>x\<close>. Higher-order unification frequently puts
+  terms into a fully \<open>\<eta>\<close>-expanded form. For example, if \<open>F\<close> has type \<open>(\<tau> \<Rightarrow> \<tau>)
+  \<Rightarrow> \<tau>\<close> then its expanded form is @{term "\<lambda>h. F (\<lambda>x. h x)"}.
 
-  Enabling @{attribute eta_contract} makes Isabelle perform \<open>\<eta>\<close>-contractions before printing, so that @{term "\<lambda>h. F (\<lambda>x. h x)"}
-  appears simply as \<open>F\<close>.
+  Enabling @{attribute eta_contract} makes Isabelle perform \<open>\<eta>\<close>-contractions
+  before printing, so that @{term "\<lambda>h. F (\<lambda>x. h x)"} appears simply as \<open>F\<close>.
 
-  Note that the distinction between a term and its \<open>\<eta>\<close>-expanded
-  form occasionally matters.  While higher-order resolution and
-  rewriting operate modulo \<open>\<alpha>\<beta>\<eta>\<close>-conversion, some other tools
-  might look at terms more discretely.
+  Note that the distinction between a term and its \<open>\<eta>\<close>-expanded form
+  occasionally matters. While higher-order resolution and rewriting operate
+  modulo \<open>\<alpha>\<beta>\<eta>\<close>-conversion, some other tools might look at terms more
+  discretely.
 
-  \<^descr> @{attribute goals_limit} controls the maximum number of
-  subgoals to be printed.
+  \<^descr> @{attribute goals_limit} controls the maximum number of subgoals to be
+  printed.
 
-  \<^descr> @{attribute show_main_goal} controls whether the main result
-  to be proven should be displayed.  This information might be
-  relevant for schematic goals, to inspect the current claim that has
-  been synthesized so far.
+  \<^descr> @{attribute show_main_goal} controls whether the main result to be proven
+  should be displayed. This information might be relevant for schematic goals,
+  to inspect the current claim that has been synthesized so far.
 
-  \<^descr> @{attribute show_hyps} controls printing of implicit
-  hypotheses of local facts.  Normally, only those hypotheses are
-  displayed that are \<^emph>\<open>not\<close> covered by the assumptions of the
-  current context: this situation indicates a fault in some tool being
-  used.
+  \<^descr> @{attribute show_hyps} controls printing of implicit hypotheses of local
+  facts. Normally, only those hypotheses are displayed that are \<^emph>\<open>not\<close> covered
+  by the assumptions of the current context: this situation indicates a fault
+  in some tool being used.
 
-  By enabling @{attribute show_hyps}, output of \<^emph>\<open>all\<close> hypotheses
-  can be enforced, which is occasionally useful for diagnostic
-  purposes.
+  By enabling @{attribute show_hyps}, output of \<^emph>\<open>all\<close> hypotheses can be
+  enforced, which is occasionally useful for diagnostic purposes.
 
-  \<^descr> @{attribute show_tags} controls printing of extra annotations
-  within theorems, such as internal position information, or the case
-  names being attached by the attribute @{attribute case_names}.
+  \<^descr> @{attribute show_tags} controls printing of extra annotations within
+  theorems, such as internal position information, or the case names being
+  attached by the attribute @{attribute case_names}.
 
-  Note that the @{attribute tagged} and @{attribute untagged}
-  attributes provide low-level access to the collection of tags
-  associated with a theorem.
+  Note that the @{attribute tagged} and @{attribute untagged} attributes
+  provide low-level access to the collection of tags associated with a
+  theorem.
 
-  \<^descr> @{attribute show_question_marks} controls printing of question
-  marks for schematic variables, such as \<open>?x\<close>.  Only the leading
-  question mark is affected, the remaining text is unchanged
-  (including proper markup for schematic variables that might be
-  relevant for user interfaces).
+  \<^descr> @{attribute show_question_marks} controls printing of question marks for
+  schematic variables, such as \<open>?x\<close>. Only the leading question mark is
+  affected, the remaining text is unchanged (including proper markup for
+  schematic variables that might be relevant for user interfaces).
 \<close>
 
 
@@ -242,62 +226,58 @@ text \<open>
     @{index_ML Print_Mode.with_modes: "string list -> ('a -> 'b) -> 'a -> 'b"} \\
   \end{mldecls}
 
-  The \<^emph>\<open>print mode\<close> facility allows to modify various operations
-  for printing.  Commands like @{command typ}, @{command term},
-  @{command thm} (see \secref{sec:print-diag}) take additional print
-  modes as optional argument.  The underlying ML operations are as
-  follows.
+  The \<^emph>\<open>print mode\<close> facility allows to modify various operations for printing.
+  Commands like @{command typ}, @{command term}, @{command thm} (see
+  \secref{sec:print-diag}) take additional print modes as optional argument.
+  The underlying ML operations are as follows.
 
-  \<^descr> @{ML "print_mode_value ()"} yields the list of currently
-  active print mode names.  This should be understood as symbolic
-  representation of certain individual features for printing (with
-  precedence from left to right).
+    \<^descr> @{ML "print_mode_value ()"} yields the list of currently active print
+    mode names. This should be understood as symbolic representation of
+    certain individual features for printing (with precedence from left to
+    right).
 
-  \<^descr> @{ML Print_Mode.with_modes}~\<open>modes f x\<close> evaluates
-  \<open>f x\<close> in an execution context where the print mode is
-  prepended by the given \<open>modes\<close>.  This provides a thread-safe
-  way to augment print modes.  It is also monotonic in the set of mode
-  names: it retains the default print mode that certain
-  user-interfaces might have installed for their proper functioning!
-
+    \<^descr> @{ML Print_Mode.with_modes}~\<open>modes f x\<close> evaluates \<open>f x\<close> in an execution
+    context where the print mode is prepended by the given \<open>modes\<close>. This
+    provides a thread-safe way to augment print modes. It is also monotonic in
+    the set of mode names: it retains the default print mode that certain
+    user-interfaces might have installed for their proper functioning!
 
   \<^medskip>
-  The pretty printer for inner syntax maintains alternative
-  mixfix productions for any print mode name invented by the user, say
-  in commands like @{command notation} or @{command abbreviation}.
-  Mode names can be arbitrary, but the following ones have a specific
-  meaning by convention:
+  The pretty printer for inner syntax maintains alternative mixfix productions
+  for any print mode name invented by the user, say in commands like @{command
+  notation} or @{command abbreviation}. Mode names can be arbitrary, but the
+  following ones have a specific meaning by convention:
 
-  \<^item> \<^verbatim>\<open>""\<close> (the empty string): default mode;
-  implicitly active as last element in the list of modes.
+    \<^item> \<^verbatim>\<open>""\<close> (the empty string): default mode; implicitly active as last
+    element in the list of modes.
 
-  \<^item> \<^verbatim>\<open>input\<close>: dummy print mode that is never active; may
-  be used to specify notation that is only available for input.
+    \<^item> \<^verbatim>\<open>input\<close>: dummy print mode that is never active; may be used to specify
+    notation that is only available for input.
 
-  \<^item> \<^verbatim>\<open>internal\<close> dummy print mode that is never active;
-  used internally in Isabelle/Pure.
+    \<^item> \<^verbatim>\<open>internal\<close> dummy print mode that is never active; used internally in
+    Isabelle/Pure.
 
-  \<^item> \<^verbatim>\<open>ASCII\<close>: prefer ASCII art over mathematical symbols.
+    \<^item> \<^verbatim>\<open>ASCII\<close>: prefer ASCII art over mathematical symbols.
 
-  \<^item> \<^verbatim>\<open>latex\<close>: additional mode that is active in {\LaTeX}
-  document preparation of Isabelle theory sources; allows to provide
-  alternative output notation.
+    \<^item> \<^verbatim>\<open>latex\<close>: additional mode that is active in {\LaTeX} document
+    preparation of Isabelle theory sources; allows to provide alternative
+    output notation.
 \<close>
 
 
 section \<open>Mixfix annotations \label{sec:mixfix}\<close>
 
-text \<open>Mixfix annotations specify concrete \<^emph>\<open>inner syntax\<close> of
-  Isabelle types and terms.  Locally fixed parameters in toplevel
-  theorem statements, locale and class specifications also admit
-  mixfix annotations in a fairly uniform manner.  A mixfix annotation
-  describes the concrete syntax, the translation to abstract
-  syntax, and the pretty printing.  Special case annotations provide a
-  simple means of specifying infix operators and binders.
+text \<open>
+  Mixfix annotations specify concrete \<^emph>\<open>inner syntax\<close> of Isabelle types and
+  terms. Locally fixed parameters in toplevel theorem statements, locale and
+  class specifications also admit mixfix annotations in a fairly uniform
+  manner. A mixfix annotation describes the concrete syntax, the translation
+  to abstract syntax, and the pretty printing. Special case annotations
+  provide a simple means of specifying infix operators and binders.
 
-  Isabelle mixfix syntax is inspired by {\OBJ} @{cite OBJ}.  It allows
-  to specify any context-free priority grammar, which is more general
-  than the fixity declarations of ML and Prolog.
+  Isabelle mixfix syntax is inspired by {\OBJ} @{cite OBJ}. It allows to
+  specify any context-free priority grammar, which is more general than the
+  fixity declarations of ML and Prolog.
 
   @{rail \<open>
     @{syntax_def mixfix}: '('
@@ -311,52 +291,48 @@ text \<open>Mixfix annotations specify concrete \<^emph>\<open>inner syntax\<clo
     prios: '[' (@{syntax nat} + ',') ']'
   \<close>}
 
-  The string given as \<open>template\<close> may include literal text,
-  spacing, blocks, and arguments (denoted by ``\<open>_\<close>''); the
-  special symbol ``\<^verbatim>\<open>\<index>\<close>'' (printed as ``\<open>\<index>\<close>'')
-  represents an index argument that specifies an implicit @{keyword
-  "structure"} reference (see also \secref{sec:locale}).  Only locally
-  fixed variables may be declared as @{keyword "structure"}.
+  The string given as \<open>template\<close> may include literal text, spacing, blocks,
+  and arguments (denoted by ``\<open>_\<close>''); the special symbol ``\<^verbatim>\<open>\<index>\<close>'' (printed as
+  ``\<open>\<index>\<close>'') represents an index argument that specifies an implicit @{keyword
+  "structure"} reference (see also \secref{sec:locale}). Only locally fixed
+  variables may be declared as @{keyword "structure"}.
 
-  Infix and binder declarations provide common abbreviations for
-  particular mixfix declarations.  So in practice, mixfix templates
-  mostly degenerate to literal text for concrete syntax, such as
-  ``\<^verbatim>\<open>++\<close>'' for an infix symbol.
+  Infix and binder declarations provide common abbreviations for particular
+  mixfix declarations. So in practice, mixfix templates mostly degenerate to
+  literal text for concrete syntax, such as ``\<^verbatim>\<open>++\<close>'' for an infix symbol.
 \<close>
 
 
 subsection \<open>The general mixfix form\<close>
 
-text \<open>In full generality, mixfix declarations work as follows.
-  Suppose a constant \<open>c :: \<tau>\<^sub>1 \<Rightarrow> \<dots> \<tau>\<^sub>n \<Rightarrow> \<tau>\<close> is annotated by
-  \<open>(mixfix [p\<^sub>1, \<dots>, p\<^sub>n] p)\<close>, where \<open>mixfix\<close> is a string
-  \<open>d\<^sub>0 _ d\<^sub>1 _ \<dots> _ d\<^sub>n\<close> consisting of delimiters that surround
-  argument positions as indicated by underscores.
+text \<open>
+  In full generality, mixfix declarations work as follows. Suppose a constant
+  \<open>c :: \<tau>\<^sub>1 \<Rightarrow> \<dots> \<tau>\<^sub>n \<Rightarrow> \<tau>\<close> is annotated by \<open>(mixfix [p\<^sub>1, \<dots>, p\<^sub>n] p)\<close>, where
+  \<open>mixfix\<close> is a string \<open>d\<^sub>0 _ d\<^sub>1 _ \<dots> _ d\<^sub>n\<close> consisting of delimiters that
+  surround argument positions as indicated by underscores.
 
-  Altogether this determines a production for a context-free priority
-  grammar, where for each argument \<open>i\<close> the syntactic category
-  is determined by \<open>\<tau>\<^sub>i\<close> (with priority \<open>p\<^sub>i\<close>), and the
-  result category is determined from \<open>\<tau>\<close> (with priority \<open>p\<close>).  Priority specifications are optional, with default 0 for
-  arguments and 1000 for the result.\<^footnote>\<open>Omitting priorities is
-  prone to syntactic ambiguities unless the delimiter tokens determine
-  fully bracketed notation, as in \<open>if _ then _ else _ fi\<close>.\<close>
+  Altogether this determines a production for a context-free priority grammar,
+  where for each argument \<open>i\<close> the syntactic category is determined by \<open>\<tau>\<^sub>i\<close>
+  (with priority \<open>p\<^sub>i\<close>), and the result category is determined from \<open>\<tau>\<close> (with
+  priority \<open>p\<close>). Priority specifications are optional, with default 0 for
+  arguments and 1000 for the result.\<^footnote>\<open>Omitting priorities is prone to
+  syntactic ambiguities unless the delimiter tokens determine fully bracketed
+  notation, as in \<open>if _ then _ else _ fi\<close>.\<close>
 
-  Since \<open>\<tau>\<close> may be again a function type, the constant
-  type scheme may have more argument positions than the mixfix
-  pattern.  Printing a nested application \<open>c t\<^sub>1 \<dots> t\<^sub>m\<close> for
-  \<open>m > n\<close> works by attaching concrete notation only to the
-  innermost part, essentially by printing \<open>(c t\<^sub>1 \<dots> t\<^sub>n) \<dots> t\<^sub>m\<close>
-  instead.  If a term has fewer arguments than specified in the mixfix
+  Since \<open>\<tau>\<close> may be again a function type, the constant type scheme may have
+  more argument positions than the mixfix pattern. Printing a nested
+  application \<open>c t\<^sub>1 \<dots> t\<^sub>m\<close> for \<open>m > n\<close> works by attaching concrete notation
+  only to the innermost part, essentially by printing \<open>(c t\<^sub>1 \<dots> t\<^sub>n) \<dots> t\<^sub>m\<close>
+  instead. If a term has fewer arguments than specified in the mixfix
   template, the concrete syntax is ignored.
 
   \<^medskip>
-  A mixfix template may also contain additional directives
-  for pretty printing, notably spaces, blocks, and breaks.  The
-  general template format is a sequence over any of the following
-  entities.
+  A mixfix template may also contain additional directives for pretty
+  printing, notably spaces, blocks, and breaks. The general template format is
+  a sequence over any of the following entities.
 
-  \<^descr> \<open>d\<close> is a delimiter, namely a non-empty sequence of
-  characters other than the following special characters:
+  \<^descr> \<open>d\<close> is a delimiter, namely a non-empty sequence of characters other than
+  the following special characters:
 
   \<^medskip>
   \begin{tabular}{ll}
@@ -369,47 +345,45 @@ text \<open>In full generality, mixfix declarations work as follows.
   \end{tabular}
   \<^medskip>
 
-  \<^descr> \<^verbatim>\<open>'\<close> escapes the special meaning of these
-  meta-characters, producing a literal version of the following
-  character, unless that is a blank.
+  \<^descr> \<^verbatim>\<open>'\<close> escapes the special meaning of these meta-characters, producing a
+  literal version of the following character, unless that is a blank.
 
-  A single quote followed by a blank separates delimiters, without
-  affecting printing, but input tokens may have additional white space
-  here.
+  A single quote followed by a blank separates delimiters, without affecting
+  printing, but input tokens may have additional white space here.
 
-  \<^descr> \<^verbatim>\<open>_\<close> is an argument position, which stands for a
-  certain syntactic category in the underlying grammar.
+  \<^descr> \<^verbatim>\<open>_\<close> is an argument position, which stands for a certain syntactic
+  category in the underlying grammar.
 
-  \<^descr> \<open>\<index>\<close> is an indexed argument position; this is the place
-  where implicit structure arguments can be attached.
+  \<^descr> \<open>\<index>\<close> is an indexed argument position; this is the place where implicit
+  structure arguments can be attached.
 
-  \<^descr> \<open>s\<close> is a non-empty sequence of spaces for printing.
-  This and the following specifications do not affect parsing at all.
+  \<^descr> \<open>s\<close> is a non-empty sequence of spaces for printing. This and the following
+  specifications do not affect parsing at all.
 
-  \<^descr> \<^verbatim>\<open>(\<close>\<open>n\<close> opens a pretty printing block.  The
-  optional number specifies how much indentation to add when a line
-  break occurs within the block.  If the parenthesis is not followed
-  by digits, the indentation defaults to 0.  A block specified via
-  \<^verbatim>\<open>(00\<close> is unbreakable.
+  \<^descr> \<^verbatim>\<open>(\<close>\<open>n\<close> opens a pretty printing block. The optional number specifies how
+  much indentation to add when a line break occurs within the block. If the
+  parenthesis is not followed by digits, the indentation defaults to 0. A
+  block specified via \<^verbatim>\<open>(00\<close> is unbreakable.
 
   \<^descr> \<^verbatim>\<open>)\<close> closes a pretty printing block.
 
   \<^descr> \<^verbatim>\<open>//\<close> forces a line break.
 
-  \<^descr> \<^verbatim>\<open>/\<close>\<open>s\<close> allows a line break.  Here \<open>s\<close>
-  stands for the string of spaces (zero or more) right after the
-  slash.  These spaces are printed if the break is \<^emph>\<open>not\<close> taken.
+  \<^descr> \<^verbatim>\<open>/\<close>\<open>s\<close> allows a line break. Here \<open>s\<close> stands for the string of spaces
+  (zero or more) right after the slash. These spaces are printed if the break
+  is \<^emph>\<open>not\<close> taken.
 
 
-  The general idea of pretty printing with blocks and breaks is also
-  described in @{cite "paulson-ml2"}; it goes back to @{cite "Oppen:1980"}.
+  The general idea of pretty printing with blocks and breaks is also described
+  in @{cite "paulson-ml2"}; it goes back to @{cite "Oppen:1980"}.
 \<close>
 
 
 subsection \<open>Infixes\<close>
 
-text \<open>Infix operators are specified by convenient short forms that
-  abbreviate general mixfix annotations as follows:
+text \<open>
+  Infix operators are specified by convenient short forms that abbreviate
+  general mixfix annotations as follows:
 
   \begin{center}
   \begin{tabular}{lll}
@@ -427,35 +401,33 @@ text \<open>Infix operators are specified by convenient short forms that
   \end{tabular}
   \end{center}
 
-  The mixfix template \<^verbatim>\<open>"(_\<close>~\<open>sy\<close>\<^verbatim>\<open>/ _)"\<close>
-  specifies two argument positions; the delimiter is preceded by a
-  space and followed by a space or line break; the entire phrase is a
-  pretty printing block.
+  The mixfix template \<^verbatim>\<open>"(_\<close>~\<open>sy\<close>\<^verbatim>\<open>/ _)"\<close> specifies two argument positions;
+  the delimiter is preceded by a space and followed by a space or line break;
+  the entire phrase is a pretty printing block.
 
-  The alternative notation \<^verbatim>\<open>op\<close>~\<open>sy\<close> is introduced
-  in addition.  Thus any infix operator may be written in prefix form
-  (as in ML), independently of the number of arguments in the term.
+  The alternative notation \<^verbatim>\<open>op\<close>~\<open>sy\<close> is introduced in addition. Thus any
+  infix operator may be written in prefix form (as in ML), independently of
+  the number of arguments in the term.
 \<close>
 
 
 subsection \<open>Binders\<close>
 
-text \<open>A \<^emph>\<open>binder\<close> is a variable-binding construct such as a
-  quantifier.  The idea to formalize \<open>\<forall>x. b\<close> as \<open>All
-  (\<lambda>x. b)\<close> for \<open>All :: ('a \<Rightarrow> bool) \<Rightarrow> bool\<close> already goes back
-  to @{cite church40}.  Isabelle declarations of certain higher-order
-  operators may be annotated with @{keyword_def "binder"} annotations
-  as follows:
+text \<open>
+  A \<^emph>\<open>binder\<close> is a variable-binding construct such as a quantifier. The idea
+  to formalize \<open>\<forall>x. b\<close> as \<open>All (\<lambda>x. b)\<close> for \<open>All :: ('a \<Rightarrow> bool) \<Rightarrow> bool\<close>
+  already goes back to @{cite church40}. Isabelle declarations of certain
+  higher-order operators may be annotated with @{keyword_def "binder"}
+  annotations as follows:
 
   \begin{center}
   \<open>c ::\<close>~\<^verbatim>\<open>"\<close>\<open>(\<tau>\<^sub>1 \<Rightarrow> \<tau>\<^sub>2) \<Rightarrow> \<tau>\<^sub>3\<close>\<^verbatim>\<open>"  (\<close>@{keyword "binder"}~\<^verbatim>\<open>"\<close>\<open>sy\<close>\<^verbatim>\<open>" [\<close>\<open>p\<close>\<^verbatim>\<open>]\<close>~\<open>q\<close>\<^verbatim>\<open>)\<close>
   \end{center}
 
-  This introduces concrete binder syntax \<open>sy x. b\<close>, where
-  \<open>x\<close> is a bound variable of type \<open>\<tau>\<^sub>1\<close>, the body \<open>b\<close> has type \<open>\<tau>\<^sub>2\<close> and the whole term has type \<open>\<tau>\<^sub>3\<close>.
-  The optional integer \<open>p\<close> specifies the syntactic priority of
-  the body; the default is \<open>q\<close>, which is also the priority of
-  the whole construct.
+  This introduces concrete binder syntax \<open>sy x. b\<close>, where \<open>x\<close> is a bound
+  variable of type \<open>\<tau>\<^sub>1\<close>, the body \<open>b\<close> has type \<open>\<tau>\<^sub>2\<close> and the whole term has
+  type \<open>\<tau>\<^sub>3\<close>. The optional integer \<open>p\<close> specifies the syntactic priority of the
+  body; the default is \<open>q\<close>, which is also the priority of the whole construct.
 
   Internally, the binder syntax is expanded to something like this:
   \begin{center}
@@ -464,17 +436,18 @@ text \<open>A \<^emph>\<open>binder\<close> is a variable-binding construct such
 
   Here @{syntax (inner) idts} is the nonterminal symbol for a list of
   identifiers with optional type constraints (see also
-  \secref{sec:pure-grammar}).  The mixfix template \<^verbatim>\<open>"(3\<close>\<open>sy\<close>\<^verbatim>\<open>_./ _)"\<close>
-  defines argument positions
-  for the bound identifiers and the body, separated by a dot with
-  optional line break; the entire phrase is a pretty printing block of
-  indentation level 3.  Note that there is no extra space after \<open>sy\<close>, so it needs to be included user specification if the binder
-  syntax ends with a token that may be continued by an identifier
-  token at the start of @{syntax (inner) idts}.
+  \secref{sec:pure-grammar}). The mixfix template \<^verbatim>\<open>"(3\<close>\<open>sy\<close>\<^verbatim>\<open>_./ _)"\<close> defines
+  argument positions for the bound identifiers and the body, separated by a
+  dot with optional line break; the entire phrase is a pretty printing block
+  of indentation level 3. Note that there is no extra space after \<open>sy\<close>, so it
+  needs to be included user specification if the binder syntax ends with a
+  token that may be continued by an identifier token at the start of @{syntax
+  (inner) idts}.
 
-  Furthermore, a syntax translation to transforms \<open>c_binder x\<^sub>1
-  \<dots> x\<^sub>n b\<close> into iterated application \<open>c (\<lambda>x\<^sub>1. \<dots> c (\<lambda>x\<^sub>n. b)\<dots>)\<close>.
-  This works in both directions, for parsing and printing.\<close>
+  Furthermore, a syntax translation to transforms \<open>c_binder x\<^sub>1 \<dots> x\<^sub>n b\<close> into
+  iterated application \<open>c (\<lambda>x\<^sub>1. \<dots> c (\<lambda>x\<^sub>n. b)\<dots>)\<close>. This works in both
+  directions, for parsing and printing.
+\<close>
 
 
 section \<open>Explicit notation \label{sec:notation}\<close>
@@ -488,12 +461,11 @@ text \<open>
     @{command_def "write"} & : & \<open>proof(state) \<rightarrow> proof(state)\<close> \\
   \end{matharray}
 
-  Commands that introduce new logical entities (terms or types)
-  usually allow to provide mixfix annotations on the spot, which is
-  convenient for default notation.  Nonetheless, the syntax may be
-  modified later on by declarations for explicit notation.  This
-  allows to add or delete mixfix annotations for of existing logical
-  entities within the current context.
+  Commands that introduce new logical entities (terms or types) usually allow
+  to provide mixfix annotations on the spot, which is convenient for default
+  notation. Nonetheless, the syntax may be modified later on by declarations
+  for explicit notation. This allows to add or delete mixfix annotations for
+  of existing logical entities within the current context.
 
   @{rail \<open>
     (@@{command type_notation} | @@{command no_type_notation}) @{syntax mode}? \<newline>
@@ -505,24 +477,22 @@ text \<open>
     @@{command write} @{syntax mode}? (@{syntax nameref} @{syntax mixfix} + @'and')
   \<close>}
 
-  \<^descr> @{command "type_notation"}~\<open>c (mx)\<close> associates mixfix
-  syntax with an existing type constructor.  The arity of the
-  constructor is retrieved from the context.
+  \<^descr> @{command "type_notation"}~\<open>c (mx)\<close> associates mixfix syntax with an
+  existing type constructor. The arity of the constructor is retrieved from
+  the context.
 
-  \<^descr> @{command "no_type_notation"} is similar to @{command
-  "type_notation"}, but removes the specified syntax annotation from
-  the present context.
+  \<^descr> @{command "no_type_notation"} is similar to @{command "type_notation"},
+  but removes the specified syntax annotation from the present context.
 
-  \<^descr> @{command "notation"}~\<open>c (mx)\<close> associates mixfix
-  syntax with an existing constant or fixed variable.  The type
-  declaration of the given entity is retrieved from the context.
+  \<^descr> @{command "notation"}~\<open>c (mx)\<close> associates mixfix syntax with an existing
+  constant or fixed variable. The type declaration of the given entity is
+  retrieved from the context.
 
-  \<^descr> @{command "no_notation"} is similar to @{command "notation"},
-  but removes the specified syntax annotation from the present
-  context.
+  \<^descr> @{command "no_notation"} is similar to @{command "notation"}, but removes
+  the specified syntax annotation from the present context.
 
-  \<^descr> @{command "write"} is similar to @{command "notation"}, but
-  works within an Isar proof body.
+  \<^descr> @{command "write"} is similar to @{command "notation"}, but works within
+  an Isar proof body.
 \<close>
 
 
@@ -530,26 +500,24 @@ section \<open>The Pure syntax \label{sec:pure-syntax}\<close>
 
 subsection \<open>Lexical matters \label{sec:inner-lex}\<close>
 
-text \<open>The inner lexical syntax vaguely resembles the outer one
-  (\secref{sec:outer-lex}), but some details are different.  There are
-  two main categories of inner syntax tokens:
+text \<open>
+  The inner lexical syntax vaguely resembles the outer one
+  (\secref{sec:outer-lex}), but some details are different. There are two main
+  categories of inner syntax tokens:
 
-  \<^enum> \<^emph>\<open>delimiters\<close> --- the literal tokens occurring in
-  productions of the given priority grammar (cf.\
-  \secref{sec:priority-grammar});
+  \<^enum> \<^emph>\<open>delimiters\<close> --- the literal tokens occurring in productions of the given
+  priority grammar (cf.\ \secref{sec:priority-grammar});
 
   \<^enum> \<^emph>\<open>named tokens\<close> --- various categories of identifiers etc.
 
 
-  Delimiters override named tokens and may thus render certain
-  identifiers inaccessible.  Sometimes the logical context admits
-  alternative ways to refer to the same entity, potentially via
-  qualified names.
+  Delimiters override named tokens and may thus render certain identifiers
+  inaccessible. Sometimes the logical context admits alternative ways to refer
+  to the same entity, potentially via qualified names.
 
   \<^medskip>
-  The categories for named tokens are defined once and for
-  all as follows, reusing some categories of the outer token syntax
-  (\secref{sec:outer-lex}).
+  The categories for named tokens are defined once and for all as follows,
+  reusing some categories of the outer token syntax (\secref{sec:outer-lex}).
 
   \begin{center}
   \begin{supertabular}{rcl}
@@ -581,32 +549,30 @@ text \<open>The inner lexical syntax vaguely resembles the outer one
 
 subsection \<open>Priority grammars \label{sec:priority-grammar}\<close>
 
-text \<open>A context-free grammar consists of a set of \<^emph>\<open>terminal
-  symbols\<close>, a set of \<^emph>\<open>nonterminal symbols\<close> and a set of
-  \<^emph>\<open>productions\<close>.  Productions have the form \<open>A = \<gamma>\<close>,
-  where \<open>A\<close> is a nonterminal and \<open>\<gamma>\<close> is a string of
-  terminals and nonterminals.  One designated nonterminal is called
-  the \<^emph>\<open>root symbol\<close>.  The language defined by the grammar
-  consists of all strings of terminals that can be derived from the
-  root symbol by applying productions as rewrite rules.
+text \<open>
+  A context-free grammar consists of a set of \<^emph>\<open>terminal symbols\<close>, a set of
+  \<^emph>\<open>nonterminal symbols\<close> and a set of \<^emph>\<open>productions\<close>. Productions have the
+  form \<open>A = \<gamma>\<close>, where \<open>A\<close> is a nonterminal and \<open>\<gamma>\<close> is a string of terminals
+  and nonterminals. One designated nonterminal is called the \<^emph>\<open>root symbol\<close>.
+  The language defined by the grammar consists of all strings of terminals
+  that can be derived from the root symbol by applying productions as rewrite
+  rules.
 
-  The standard Isabelle parser for inner syntax uses a \<^emph>\<open>priority
-  grammar\<close>.  Each nonterminal is decorated by an integer priority:
-  \<open>A\<^sup>(\<^sup>p\<^sup>)\<close>.  In a derivation, \<open>A\<^sup>(\<^sup>p\<^sup>)\<close> may be rewritten
-  using a production \<open>A\<^sup>(\<^sup>q\<^sup>) = \<gamma>\<close> only if \<open>p \<le> q\<close>.  Any
-  priority grammar can be translated into a normal context-free
-  grammar by introducing new nonterminals and productions.
+  The standard Isabelle parser for inner syntax uses a \<^emph>\<open>priority grammar\<close>.
+  Each nonterminal is decorated by an integer priority: \<open>A\<^sup>(\<^sup>p\<^sup>)\<close>. In a
+  derivation, \<open>A\<^sup>(\<^sup>p\<^sup>)\<close> may be rewritten using a production \<open>A\<^sup>(\<^sup>q\<^sup>) = \<gamma>\<close> only
+  if \<open>p \<le> q\<close>. Any priority grammar can be translated into a normal
+  context-free grammar by introducing new nonterminals and productions.
 
   \<^medskip>
-  Formally, a set of context free productions \<open>G\<close>
-  induces a derivation relation \<open>\<longrightarrow>\<^sub>G\<close> as follows.  Let \<open>\<alpha>\<close> and \<open>\<beta>\<close> denote strings of terminal or nonterminal symbols.
-  Then \<open>\<alpha> A\<^sup>(\<^sup>p\<^sup>) \<beta> \<longrightarrow>\<^sub>G \<alpha> \<gamma> \<beta>\<close> holds if and only if \<open>G\<close>
+  Formally, a set of context free productions \<open>G\<close> induces a derivation
+  relation \<open>\<longrightarrow>\<^sub>G\<close> as follows. Let \<open>\<alpha>\<close> and \<open>\<beta>\<close> denote strings of terminal or
+  nonterminal symbols. Then \<open>\<alpha> A\<^sup>(\<^sup>p\<^sup>) \<beta> \<longrightarrow>\<^sub>G \<alpha> \<gamma> \<beta>\<close> holds if and only if \<open>G\<close>
   contains some production \<open>A\<^sup>(\<^sup>q\<^sup>) = \<gamma>\<close> for \<open>p \<le> q\<close>.
 
   \<^medskip>
-  The following grammar for arithmetic expressions
-  demonstrates how binding power and associativity of operators can be
-  enforced by priorities.
+  The following grammar for arithmetic expressions demonstrates how binding
+  power and associativity of operators can be enforced by priorities.
 
   \begin{center}
   \begin{tabular}{rclr}
@@ -617,28 +583,25 @@ text \<open>A context-free grammar consists of a set of \<^emph>\<open>terminal
   \<open>A\<^sup>(\<^sup>3\<^sup>)\<close> & \<open>=\<close> & \<^verbatim>\<open>-\<close> \<open>A\<^sup>(\<^sup>3\<^sup>)\<close> \\
   \end{tabular}
   \end{center}
-  The choice of priorities determines that \<^verbatim>\<open>-\<close> binds
-  tighter than \<^verbatim>\<open>*\<close>, which binds tighter than \<^verbatim>\<open>+\<close>.
-  Furthermore \<^verbatim>\<open>+\<close> associates to the left and
-  \<^verbatim>\<open>*\<close> to the right.
+  The choice of priorities determines that \<^verbatim>\<open>-\<close> binds tighter than \<^verbatim>\<open>*\<close>, which
+  binds tighter than \<^verbatim>\<open>+\<close>. Furthermore \<^verbatim>\<open>+\<close> associates to the left and \<^verbatim>\<open>*\<close> to
+  the right.
 
   \<^medskip>
   For clarity, grammars obey these conventions:
 
-  \<^item> All priorities must lie between 0 and 1000.
+    \<^item> All priorities must lie between 0 and 1000.
 
-  \<^item> Priority 0 on the right-hand side and priority 1000 on the
-  left-hand side may be omitted.
+    \<^item> Priority 0 on the right-hand side and priority 1000 on the left-hand
+    side may be omitted.
 
-  \<^item> The production \<open>A\<^sup>(\<^sup>p\<^sup>) = \<alpha>\<close> is written as \<open>A = \<alpha>
-  (p)\<close>, i.e.\ the priority of the left-hand side actually appears in
-  a column on the far right.
+    \<^item> The production \<open>A\<^sup>(\<^sup>p\<^sup>) = \<alpha>\<close> is written as \<open>A = \<alpha> (p)\<close>, i.e.\ the
+    priority of the left-hand side actually appears in a column on the far
+    right.
 
-  \<^item> Alternatives are separated by \<open>|\<close>.
+    \<^item> Alternatives are separated by \<open>|\<close>.
 
-  \<^item> Repetition is indicated by dots \<open>(\<dots>)\<close> in an informal
-  but obvious way.
-
+    \<^item> Repetition is indicated by dots \<open>(\<dots>)\<close> in an informal but obvious way.
 
   Using these conventions, the example grammar specification above
   takes the form:
@@ -656,8 +619,9 @@ text \<open>A context-free grammar consists of a set of \<^emph>\<open>terminal
 
 subsection \<open>The Pure grammar \label{sec:pure-grammar}\<close>
 
-text \<open>The priority grammar of the \<open>Pure\<close> theory is defined
-  approximately like this:
+text \<open>
+  The priority grammar of the \<open>Pure\<close> theory is defined approximately like
+  this:
 
   \begin{center}
   \begin{supertabular}{rclr}
@@ -729,55 +693,54 @@ text \<open>The priority grammar of the \<open>Pure\<close> theory is defined
   \end{center}
 
   \<^medskip>
-  Here literal terminals are printed \<^verbatim>\<open>verbatim\<close>;
-  see also \secref{sec:inner-lex} for further token categories of the
-  inner syntax.  The meaning of the nonterminals defined by the above
-  grammar is as follows:
+  Here literal terminals are printed \<^verbatim>\<open>verbatim\<close>; see also
+  \secref{sec:inner-lex} for further token categories of the inner syntax. The
+  meaning of the nonterminals defined by the above grammar is as follows:
 
   \<^descr> @{syntax_ref (inner) any} denotes any term.
 
-  \<^descr> @{syntax_ref (inner) prop} denotes meta-level propositions,
-  which are terms of type @{typ prop}.  The syntax of such formulae of
-  the meta-logic is carefully distinguished from usual conventions for
-  object-logics.  In particular, plain \<open>\<lambda>\<close>-term notation is
-  \<^emph>\<open>not\<close> recognized as @{syntax (inner) prop}.
+  \<^descr> @{syntax_ref (inner) prop} denotes meta-level propositions, which are
+  terms of type @{typ prop}. The syntax of such formulae of the meta-logic is
+  carefully distinguished from usual conventions for object-logics. In
+  particular, plain \<open>\<lambda>\<close>-term notation is \<^emph>\<open>not\<close> recognized as @{syntax (inner)
+  prop}.
 
-  \<^descr> @{syntax_ref (inner) aprop} denotes atomic propositions, which
-  are embedded into regular @{syntax (inner) prop} by means of an
-  explicit \<^verbatim>\<open>PROP\<close> token.
+  \<^descr> @{syntax_ref (inner) aprop} denotes atomic propositions, which are
+  embedded into regular @{syntax (inner) prop} by means of an explicit \<^verbatim>\<open>PROP\<close>
+  token.
 
-  Terms of type @{typ prop} with non-constant head, e.g.\ a plain
-  variable, are printed in this form.  Constants that yield type @{typ
-  prop} are expected to provide their own concrete syntax; otherwise
-  the printed version will appear like @{syntax (inner) logic} and
-  cannot be parsed again as @{syntax (inner) prop}.
+  Terms of type @{typ prop} with non-constant head, e.g.\ a plain variable,
+  are printed in this form. Constants that yield type @{typ prop} are expected
+  to provide their own concrete syntax; otherwise the printed version will
+  appear like @{syntax (inner) logic} and cannot be parsed again as @{syntax
+  (inner) prop}.
 
-  \<^descr> @{syntax_ref (inner) logic} denotes arbitrary terms of a
-  logical type, excluding type @{typ prop}.  This is the main
-  syntactic category of object-logic entities, covering plain \<open>\<lambda>\<close>-term notation (variables, abstraction, application), plus
-  anything defined by the user.
+  \<^descr> @{syntax_ref (inner) logic} denotes arbitrary terms of a logical type,
+  excluding type @{typ prop}. This is the main syntactic category of
+  object-logic entities, covering plain \<open>\<lambda>\<close>-term notation (variables,
+  abstraction, application), plus anything defined by the user.
 
-  When specifying notation for logical entities, all logical types
-  (excluding @{typ prop}) are \<^emph>\<open>collapsed\<close> to this single category
-  of @{syntax (inner) logic}.
+  When specifying notation for logical entities, all logical types (excluding
+  @{typ prop}) are \<^emph>\<open>collapsed\<close> to this single category of @{syntax (inner)
+  logic}.
 
-  \<^descr> @{syntax_ref (inner) index} denotes an optional index term for
-  indexed syntax.  If omitted, it refers to the first @{keyword_ref
-  "structure"} variable in the context.  The special dummy ``\<open>\<index>\<close>'' serves as pattern variable in mixfix annotations that
-  introduce indexed notation.
+  \<^descr> @{syntax_ref (inner) index} denotes an optional index term for indexed
+  syntax. If omitted, it refers to the first @{keyword_ref "structure"}
+  variable in the context. The special dummy ``\<open>\<index>\<close>'' serves as pattern
+  variable in mixfix annotations that introduce indexed notation.
 
-  \<^descr> @{syntax_ref (inner) idt} denotes identifiers, possibly
-  constrained by types.
+  \<^descr> @{syntax_ref (inner) idt} denotes identifiers, possibly constrained by
+  types.
 
-  \<^descr> @{syntax_ref (inner) idts} denotes a sequence of @{syntax_ref
-  (inner) idt}.  This is the most basic category for variables in
-  iterated binders, such as \<open>\<lambda>\<close> or \<open>\<And>\<close>.
+  \<^descr> @{syntax_ref (inner) idts} denotes a sequence of @{syntax_ref (inner)
+  idt}. This is the most basic category for variables in iterated binders,
+  such as \<open>\<lambda>\<close> or \<open>\<And>\<close>.
 
-  \<^descr> @{syntax_ref (inner) pttrn} and @{syntax_ref (inner) pttrns}
-  denote patterns for abstraction, cases bindings etc.  In Pure, these
-  categories start as a merely copy of @{syntax (inner) idt} and
-  @{syntax (inner) idts}, respectively.  Object-logics may add
-  additional productions for binding forms.
+  \<^descr> @{syntax_ref (inner) pttrn} and @{syntax_ref (inner) pttrns} denote
+  patterns for abstraction, cases bindings etc. In Pure, these categories
+  start as a merely copy of @{syntax (inner) idt} and @{syntax (inner) idts},
+  respectively. Object-logics may add additional productions for binding
+  forms.
 
   \<^descr> @{syntax_ref (inner) type} denotes types of the meta-logic.
 
@@ -786,58 +749,52 @@ text \<open>The priority grammar of the \<open>Pure\<close> theory is defined
 
   Here are some further explanations of certain syntax features.
 
-  \<^item> In @{syntax (inner) idts}, note that \<open>x :: nat y\<close> is
-  parsed as \<open>x :: (nat y)\<close>, treating \<open>y\<close> like a type
-  constructor applied to \<open>nat\<close>.  To avoid this interpretation,
-  write \<open>(x :: nat) y\<close> with explicit parentheses.
+  \<^item> In @{syntax (inner) idts}, note that \<open>x :: nat y\<close> is parsed as \<open>x :: (nat
+  y)\<close>, treating \<open>y\<close> like a type constructor applied to \<open>nat\<close>. To avoid this
+  interpretation, write \<open>(x :: nat) y\<close> with explicit parentheses.
 
-  \<^item> Similarly, \<open>x :: nat y :: nat\<close> is parsed as \<open>x ::
-  (nat y :: nat)\<close>.  The correct form is \<open>(x :: nat) (y ::
-  nat)\<close>, or \<open>(x :: nat) y :: nat\<close> if \<open>y\<close> is last in the
-  sequence of identifiers.
+  \<^item> Similarly, \<open>x :: nat y :: nat\<close> is parsed as \<open>x :: (nat y :: nat)\<close>. The
+  correct form is \<open>(x :: nat) (y :: nat)\<close>, or \<open>(x :: nat) y :: nat\<close> if \<open>y\<close> is
+  last in the sequence of identifiers.
 
-  \<^item> Type constraints for terms bind very weakly.  For example,
-  \<open>x < y :: nat\<close> is normally parsed as \<open>(x < y) ::
-  nat\<close>, unless \<open><\<close> has a very low priority, in which case the
-  input is likely to be ambiguous.  The correct form is \<open>x < (y
-  :: nat)\<close>.
+  \<^item> Type constraints for terms bind very weakly. For example, \<open>x < y :: nat\<close>
+  is normally parsed as \<open>(x < y) :: nat\<close>, unless \<open><\<close> has a very low priority,
+  in which case the input is likely to be ambiguous. The correct form is \<open>x <
+  (y :: nat)\<close>.
 
   \<^item> Dummy variables (written as underscore) may occur in different
   roles.
 
-    \<^descr> A type ``\<open>_\<close>'' or ``\<open>_ :: sort\<close>'' acts like an
-    anonymous inference parameter, which is filled-in according to the
-    most general type produced by the type-checking phase.
+    \<^descr> A type ``\<open>_\<close>'' or ``\<open>_ :: sort\<close>'' acts like an anonymous inference
+    parameter, which is filled-in according to the most general type produced
+    by the type-checking phase.
 
-    \<^descr> A bound ``\<open>_\<close>'' refers to a vacuous abstraction, where
-    the body does not refer to the binding introduced here.  As in the
-    term @{term "\<lambda>x _. x"}, which is \<open>\<alpha>\<close>-equivalent to \<open>\<lambda>x y. x\<close>.
+    \<^descr> A bound ``\<open>_\<close>'' refers to a vacuous abstraction, where the body does not
+    refer to the binding introduced here. As in the term @{term "\<lambda>x _. x"},
+    which is \<open>\<alpha>\<close>-equivalent to \<open>\<lambda>x y. x\<close>.
 
-    \<^descr> A free ``\<open>_\<close>'' refers to an implicit outer binding.
-    Higher definitional packages usually allow forms like \<open>f x _
-    = x\<close>.
+    \<^descr> A free ``\<open>_\<close>'' refers to an implicit outer binding. Higher definitional
+    packages usually allow forms like \<open>f x _ = x\<close>.
 
-    \<^descr> A schematic ``\<open>_\<close>'' (within a term pattern, see
-    \secref{sec:term-decls}) refers to an anonymous variable that is
-    implicitly abstracted over its context of locally bound variables.
-    For example, this allows pattern matching of \<open>{x. f x = g
-    x}\<close> against \<open>{x. _ = _}\<close>, or even \<open>{_. _ = _}\<close> by
+    \<^descr> A schematic ``\<open>_\<close>'' (within a term pattern, see \secref{sec:term-decls})
+    refers to an anonymous variable that is implicitly abstracted over its
+    context of locally bound variables. For example, this allows pattern
+    matching of \<open>{x. f x = g x}\<close> against \<open>{x. _ = _}\<close>, or even \<open>{_. _ = _}\<close> by
     using both bound and schematic dummies.
 
-  \<^descr> The three literal dots ``\<^verbatim>\<open>...\<close>'' may be also
-  written as ellipsis symbol \<^verbatim>\<open>\<dots>\<close>.  In both cases this
-  refers to a special schematic variable, which is bound in the
-  context.  This special term abbreviation works nicely with
+  \<^descr> The three literal dots ``\<^verbatim>\<open>...\<close>'' may be also written as ellipsis symbol
+  \<^verbatim>\<open>\<dots>\<close>. In both cases this refers to a special schematic variable, which is
+  bound in the context. This special term abbreviation works nicely with
   calculational reasoning (\secref{sec:calculation}).
 
-  \<^descr> \<^verbatim>\<open>CONST\<close> ensures that the given identifier is treated
-  as constant term, and passed through the parse tree in fully
-  internalized form.  This is particularly relevant for translation
-  rules (\secref{sec:syn-trans}), notably on the RHS.
+  \<^descr> \<^verbatim>\<open>CONST\<close> ensures that the given identifier is treated as constant term,
+  and passed through the parse tree in fully internalized form. This is
+  particularly relevant for translation rules (\secref{sec:syn-trans}),
+  notably on the RHS.
 
-  \<^descr> \<^verbatim>\<open>XCONST\<close> is similar to \<^verbatim>\<open>CONST\<close>, but
-  retains the constant name as given.  This is only relevant to
-  translation rules (\secref{sec:syn-trans}), notably on the LHS.
+  \<^descr> \<^verbatim>\<open>XCONST\<close> is similar to \<^verbatim>\<open>CONST\<close>, but retains the constant name as given.
+  This is only relevant to translation rules (\secref{sec:syn-trans}), notably
+  on the LHS.
 \<close>
 
 
@@ -848,46 +805,45 @@ text \<open>
     @{command_def "print_syntax"}\<open>\<^sup>*\<close> & : & \<open>context \<rightarrow>\<close> \\
   \end{matharray}
 
-  \<^descr> @{command "print_syntax"} prints the inner syntax of the
-  current context.  The output can be quite large; the most important
-  sections are explained below.
+  \<^descr> @{command "print_syntax"} prints the inner syntax of the current context.
+  The output can be quite large; the most important sections are explained
+  below.
 
-    \<^descr> \<open>lexicon\<close> lists the delimiters of the inner token
-    language; see \secref{sec:inner-lex}.
+    \<^descr> \<open>lexicon\<close> lists the delimiters of the inner token language; see
+    \secref{sec:inner-lex}.
 
-    \<^descr> \<open>prods\<close> lists the productions of the underlying
-    priority grammar; see \secref{sec:priority-grammar}.
+    \<^descr> \<open>prods\<close> lists the productions of the underlying priority grammar; see
+    \secref{sec:priority-grammar}.
 
-    The nonterminal \<open>A\<^sup>(\<^sup>p\<^sup>)\<close> is rendered in plain text as \<open>A[p]\<close>; delimiters are quoted.  Many productions have an extra
-    \<open>\<dots> => name\<close>.  These names later become the heads of parse
-    trees; they also guide the pretty printer.
+    The nonterminal \<open>A\<^sup>(\<^sup>p\<^sup>)\<close> is rendered in plain text as \<open>A[p]\<close>; delimiters
+    are quoted. Many productions have an extra \<open>\<dots> => name\<close>. These names later
+    become the heads of parse trees; they also guide the pretty printer.
 
-    Productions without such parse tree names are called \<^emph>\<open>copy
-    productions\<close>.  Their right-hand side must have exactly one
-    nonterminal symbol (or named token).  The parser does not create a
-    new parse tree node for copy productions, but simply returns the
-    parse tree of the right-hand symbol.
+    Productions without such parse tree names are called \<^emph>\<open>copy productions\<close>.
+    Their right-hand side must have exactly one nonterminal symbol (or named
+    token). The parser does not create a new parse tree node for copy
+    productions, but simply returns the parse tree of the right-hand symbol.
 
     If the right-hand side of a copy production consists of a single
     nonterminal without any delimiters, then it is called a \<^emph>\<open>chain
-    production\<close>.  Chain productions act as abbreviations: conceptually,
-    they are removed from the grammar by adding new productions.
-    Priority information attached to chain productions is ignored; only
-    the dummy value \<open>-1\<close> is displayed.
+    production\<close>. Chain productions act as abbreviations: conceptually, they
+    are removed from the grammar by adding new productions. Priority
+    information attached to chain productions is ignored; only the dummy value
+    \<open>-1\<close> is displayed.
 
-    \<^descr> \<open>print modes\<close> lists the alternative print modes
-    provided by this grammar; see \secref{sec:print-modes}.
+    \<^descr> \<open>print modes\<close> lists the alternative print modes provided by this
+    grammar; see \secref{sec:print-modes}.
 
-    \<^descr> \<open>parse_rules\<close> and \<open>print_rules\<close> relate to
-    syntax translations (macros); see \secref{sec:syn-trans}.
+    \<^descr> \<open>parse_rules\<close> and \<open>print_rules\<close> relate to syntax translations (macros);
+    see \secref{sec:syn-trans}.
 
-    \<^descr> \<open>parse_ast_translation\<close> and \<open>print_ast_translation\<close> list sets of constants that invoke
-    translation functions for abstract syntax trees, which are only
-    required in very special situations; see \secref{sec:tr-funs}.
+    \<^descr> \<open>parse_ast_translation\<close> and \<open>print_ast_translation\<close> list sets of
+    constants that invoke translation functions for abstract syntax trees,
+    which are only required in very special situations; see
+    \secref{sec:tr-funs}.
 
-    \<^descr> \<open>parse_translation\<close> and \<open>print_translation\<close>
-    list the sets of constants that invoke regular translation
-    functions; see \secref{sec:tr-funs}.
+    \<^descr> \<open>parse_translation\<close> and \<open>print_translation\<close> list the sets of constants
+    that invoke regular translation functions; see \secref{sec:tr-funs}.
 \<close>
 
 
@@ -899,37 +855,36 @@ text \<open>
     @{attribute_def syntax_ambiguity_limit} & : & \<open>attribute\<close> & default \<open>10\<close> \\
   \end{tabular}
 
-  Depending on the grammar and the given input, parsing may be
-  ambiguous.  Isabelle lets the Earley parser enumerate all possible
-  parse trees, and then tries to make the best out of the situation.
-  Terms that cannot be type-checked are filtered out, which often
-  leads to a unique result in the end.  Unlike regular type
-  reconstruction, which is applied to the whole collection of input
-  terms simultaneously, the filtering stage only treats each given
-  term in isolation.  Filtering is also not attempted for individual
+  Depending on the grammar and the given input, parsing may be ambiguous.
+  Isabelle lets the Earley parser enumerate all possible parse trees, and then
+  tries to make the best out of the situation. Terms that cannot be
+  type-checked are filtered out, which often leads to a unique result in the
+  end. Unlike regular type reconstruction, which is applied to the whole
+  collection of input terms simultaneously, the filtering stage only treats
+  each given term in isolation. Filtering is also not attempted for individual
   types or raw ASTs (as required for @{command translations}).
 
-  Certain warning or error messages are printed, depending on the
-  situation and the given configuration options.  Parsing ultimately
-  fails, if multiple results remain after the filtering phase.
+  Certain warning or error messages are printed, depending on the situation
+  and the given configuration options. Parsing ultimately fails, if multiple
+  results remain after the filtering phase.
 
-  \<^descr> @{attribute syntax_ambiguity_warning} controls output of
-  explicit warning messages about syntax ambiguity.
+  \<^descr> @{attribute syntax_ambiguity_warning} controls output of explicit warning
+  messages about syntax ambiguity.
 
-  \<^descr> @{attribute syntax_ambiguity_limit} determines the number of
-  resulting parse trees that are shown as part of the printed message
-  in case of an ambiguity.
+  \<^descr> @{attribute syntax_ambiguity_limit} determines the number of resulting
+  parse trees that are shown as part of the printed message in case of an
+  ambiguity.
 \<close>
 
 
 section \<open>Syntax transformations \label{sec:syntax-transformations}\<close>
 
-text \<open>The inner syntax engine of Isabelle provides separate
-  mechanisms to transform parse trees either via rewrite systems on
-  first-order ASTs (\secref{sec:syn-trans}), or ML functions on ASTs
-  or syntactic \<open>\<lambda>\<close>-terms (\secref{sec:tr-funs}).  This works
-  both for parsing and printing, as outlined in
-  \figref{fig:parse-print}.
+text \<open>
+  The inner syntax engine of Isabelle provides separate mechanisms to
+  transform parse trees either via rewrite systems on first-order ASTs
+  (\secref{sec:syn-trans}), or ML functions on ASTs or syntactic \<open>\<lambda>\<close>-terms
+  (\secref{sec:tr-funs}). This works both for parsing and printing, as
+  outlined in \figref{fig:parse-print}.
 
   \begin{figure}[htbp]
   \begin{center}
@@ -954,137 +909,129 @@ text \<open>The inner syntax engine of Isabelle provides separate
   \caption{Parsing and printing with translations}\label{fig:parse-print}
   \end{figure}
 
-  These intermediate syntax tree formats eventually lead to a pre-term
-  with all names and binding scopes resolved, but most type
-  information still missing.  Explicit type constraints might be given by
-  the user, or implicit position information by the system --- both
-  need to be passed-through carefully by syntax transformations.
+  These intermediate syntax tree formats eventually lead to a pre-term with
+  all names and binding scopes resolved, but most type information still
+  missing. Explicit type constraints might be given by the user, or implicit
+  position information by the system --- both need to be passed-through
+  carefully by syntax transformations.
 
-  Pre-terms are further processed by the so-called \<^emph>\<open>check\<close> and
-  \<^emph>\<open>uncheck\<close> phases that are intertwined with type-inference (see
-  also @{cite "isabelle-implementation"}).  The latter allows to operate
-  on higher-order abstract syntax with proper binding and type
-  information already available.
+  Pre-terms are further processed by the so-called \<^emph>\<open>check\<close> and \<^emph>\<open>uncheck\<close>
+  phases that are intertwined with type-inference (see also @{cite
+  "isabelle-implementation"}). The latter allows to operate on higher-order
+  abstract syntax with proper binding and type information already available.
 
-  As a rule of thumb, anything that manipulates bindings of variables
-  or constants needs to be implemented as syntax transformation (see
-  below).  Anything else is better done via check/uncheck: a prominent
-  example application is the @{command abbreviation} concept of
-  Isabelle/Pure.\<close>
+  As a rule of thumb, anything that manipulates bindings of variables or
+  constants needs to be implemented as syntax transformation (see below).
+  Anything else is better done via check/uncheck: a prominent example
+  application is the @{command abbreviation} concept of Isabelle/Pure.
+\<close>
 
 
 subsection \<open>Abstract syntax trees \label{sec:ast}\<close>
 
-text \<open>The ML datatype @{ML_type Ast.ast} explicitly represents the
-  intermediate AST format that is used for syntax rewriting
-  (\secref{sec:syn-trans}).  It is defined in ML as follows:
+text \<open>
+  The ML datatype @{ML_type Ast.ast} explicitly represents the intermediate
+  AST format that is used for syntax rewriting (\secref{sec:syn-trans}). It is
+  defined in ML as follows:
   @{verbatim [display]
 \<open>datatype ast =
   Constant of string |
   Variable of string |
   Appl of ast list\<close>}
 
-  An AST is either an atom (constant or variable) or a list of (at
-  least two) subtrees.  Occasional diagnostic output of ASTs uses
-  notation that resembles S-expression of LISP.  Constant atoms are
-  shown as quoted strings, variable atoms as non-quoted strings and
-  applications as a parenthesized list of subtrees.  For example, the
-  AST
+  An AST is either an atom (constant or variable) or a list of (at least two)
+  subtrees. Occasional diagnostic output of ASTs uses notation that resembles
+  S-expression of LISP. Constant atoms are shown as quoted strings, variable
+  atoms as non-quoted strings and applications as a parenthesized list of
+  subtrees. For example, the AST
   @{ML [display] \<open>Ast.Appl [Ast.Constant "_abs", Ast.Variable "x", Ast.Variable "t"]\<close>}
-  is pretty-printed as \<^verbatim>\<open>("_abs" x t)\<close>.  Note that
-  \<^verbatim>\<open>()\<close> and \<^verbatim>\<open>(x)\<close> are excluded as ASTs, because
-  they have too few subtrees.
+  is pretty-printed as \<^verbatim>\<open>("_abs" x t)\<close>. Note that \<^verbatim>\<open>()\<close> and \<^verbatim>\<open>(x)\<close> are
+  excluded as ASTs, because they have too few subtrees.
 
   \<^medskip>
-  AST application is merely a pro-forma mechanism to indicate
-  certain syntactic structures.  Thus \<^verbatim>\<open>(c a b)\<close> could mean
-  either term application or type application, depending on the
-  syntactic context.
+  AST application is merely a pro-forma mechanism to indicate certain
+  syntactic structures. Thus \<^verbatim>\<open>(c a b)\<close> could mean either term application or
+  type application, depending on the syntactic context.
 
-  Nested application like \<^verbatim>\<open>(("_abs" x t) u)\<close> is also
-  possible, but ASTs are definitely first-order: the syntax constant
-  \<^verbatim>\<open>"_abs"\<close> does not bind the \<^verbatim>\<open>x\<close> in any way.
-  Proper bindings are introduced in later stages of the term syntax,
-  where \<^verbatim>\<open>("_abs" x t)\<close> becomes an @{ML Abs} node and
-  occurrences of \<^verbatim>\<open>x\<close> in \<^verbatim>\<open>t\<close> are replaced by bound
-  variables (represented as de-Bruijn indices).
+  Nested application like \<^verbatim>\<open>(("_abs" x t) u)\<close> is also possible, but ASTs are
+  definitely first-order: the syntax constant \<^verbatim>\<open>"_abs"\<close> does not bind the \<^verbatim>\<open>x\<close>
+  in any way. Proper bindings are introduced in later stages of the term
+  syntax, where \<^verbatim>\<open>("_abs" x t)\<close> becomes an @{ML Abs} node and occurrences of
+  \<^verbatim>\<open>x\<close> in \<^verbatim>\<open>t\<close> are replaced by bound variables (represented as de-Bruijn
+  indices).
 \<close>
 
 
 subsubsection \<open>AST constants versus variables\<close>
 
-text \<open>Depending on the situation --- input syntax, output syntax,
-  translation patterns --- the distinction of atomic ASTs as @{ML
-  Ast.Constant} versus @{ML Ast.Variable} serves slightly different
-  purposes.
+text \<open>
+  Depending on the situation --- input syntax, output syntax, translation
+  patterns --- the distinction of atomic ASTs as @{ML Ast.Constant} versus
+  @{ML Ast.Variable} serves slightly different purposes.
 
-  Input syntax of a term such as \<open>f a b = c\<close> does not yet
-  indicate the scopes of atomic entities \<open>f, a, b, c\<close>: they
-  could be global constants or local variables, even bound ones
-  depending on the context of the term.  @{ML Ast.Variable} leaves
-  this choice still open: later syntax layers (or translation
-  functions) may capture such a variable to determine its role
-  specifically, to make it a constant, bound variable, free variable
-  etc.  In contrast, syntax translations that introduce already known
-  constants would rather do it via @{ML Ast.Constant} to prevent
-  accidental re-interpretation later on.
+  Input syntax of a term such as \<open>f a b = c\<close> does not yet indicate the scopes
+  of atomic entities \<open>f, a, b, c\<close>: they could be global constants or local
+  variables, even bound ones depending on the context of the term. @{ML
+  Ast.Variable} leaves this choice still open: later syntax layers (or
+  translation functions) may capture such a variable to determine its role
+  specifically, to make it a constant, bound variable, free variable etc. In
+  contrast, syntax translations that introduce already known constants would
+  rather do it via @{ML Ast.Constant} to prevent accidental re-interpretation
+  later on.
 
-  Output syntax turns term constants into @{ML Ast.Constant} and
-  variables (free or schematic) into @{ML Ast.Variable}.  This
-  information is precise when printing fully formal \<open>\<lambda>\<close>-terms.
+  Output syntax turns term constants into @{ML Ast.Constant} and variables
+  (free or schematic) into @{ML Ast.Variable}. This information is precise
+  when printing fully formal \<open>\<lambda>\<close>-terms.
 
   \<^medskip>
-  AST translation patterns (\secref{sec:syn-trans}) that
-  represent terms cannot distinguish constants and variables
-  syntactically.  Explicit indication of \<open>CONST c\<close> inside the
-  term language is required, unless \<open>c\<close> is known as special
-  \<^emph>\<open>syntax constant\<close> (see also @{command syntax}).  It is also
-  possible to use @{command syntax} declarations (without mixfix
-  annotation) to enforce that certain unqualified names are always
-  treated as constant within the syntax machinery.
+  AST translation patterns (\secref{sec:syn-trans}) that represent terms
+  cannot distinguish constants and variables syntactically. Explicit
+  indication of \<open>CONST c\<close> inside the term language is required, unless \<open>c\<close> is
+  known as special \<^emph>\<open>syntax constant\<close> (see also @{command syntax}). It is also
+  possible to use @{command syntax} declarations (without mixfix annotation)
+  to enforce that certain unqualified names are always treated as constant
+  within the syntax machinery.
 
-  The situation is simpler for ASTs that represent types or sorts,
-  since the concrete syntax already distinguishes type variables from
-  type constants (constructors).  So \<open>('a, 'b) foo\<close>
-  corresponds to an AST application of some constant for \<open>foo\<close>
-  and variable arguments for \<open>'a\<close> and \<open>'b\<close>.  Note that
-  the postfix application is merely a feature of the concrete syntax,
-  while in the AST the constructor occurs in head position.\<close>
+  The situation is simpler for ASTs that represent types or sorts, since the
+  concrete syntax already distinguishes type variables from type constants
+  (constructors). So \<open>('a, 'b) foo\<close> corresponds to an AST application of some
+  constant for \<open>foo\<close> and variable arguments for \<open>'a\<close> and \<open>'b\<close>. Note that the
+  postfix application is merely a feature of the concrete syntax, while in the
+  AST the constructor occurs in head position.
+\<close>
 
 
 subsubsection \<open>Authentic syntax names\<close>
 
-text \<open>Naming constant entities within ASTs is another delicate
-  issue.  Unqualified names are resolved in the name space tables in
-  the last stage of parsing, after all translations have been applied.
-  Since syntax transformations do not know about this later name
-  resolution, there can be surprises in boundary cases.
+text \<open>
+  Naming constant entities within ASTs is another delicate issue. Unqualified
+  names are resolved in the name space tables in the last stage of parsing,
+  after all translations have been applied. Since syntax transformations do
+  not know about this later name resolution, there can be surprises in
+  boundary cases.
 
-  \<^emph>\<open>Authentic syntax names\<close> for @{ML Ast.Constant} avoid this
-  problem: the fully-qualified constant name with a special prefix for
-  its formal category (\<open>class\<close>, \<open>type\<close>, \<open>const\<close>, \<open>fixed\<close>) represents the information faithfully
-  within the untyped AST format.  Accidental overlap with free or
-  bound variables is excluded as well.  Authentic syntax names work
-  implicitly in the following situations:
+  \<^emph>\<open>Authentic syntax names\<close> for @{ML Ast.Constant} avoid this problem: the
+  fully-qualified constant name with a special prefix for its formal category
+  (\<open>class\<close>, \<open>type\<close>, \<open>const\<close>, \<open>fixed\<close>) represents the information faithfully
+  within the untyped AST format. Accidental overlap with free or bound
+  variables is excluded as well. Authentic syntax names work implicitly in the
+  following situations:
 
-  \<^item> Input of term constants (or fixed variables) that are
-  introduced by concrete syntax via @{command notation}: the
-  correspondence of a particular grammar production to some known term
-  entity is preserved.
+    \<^item> Input of term constants (or fixed variables) that are introduced by
+    concrete syntax via @{command notation}: the correspondence of a
+    particular grammar production to some known term entity is preserved.
 
-  \<^item> Input of type constants (constructors) and type classes ---
-  thanks to explicit syntactic distinction independently on the
-  context.
+    \<^item> Input of type constants (constructors) and type classes --- thanks to
+    explicit syntactic distinction independently on the context.
 
-  \<^item> Output of term constants, type constants, type classes ---
-  this information is already available from the internal term to be
-  printed.
+    \<^item> Output of term constants, type constants, type classes --- this
+    information is already available from the internal term to be printed.
 
-
-  In other words, syntax transformations that operate on input terms
-  written as prefix applications are difficult to make robust.
-  Luckily, this case rarely occurs in practice, because syntax forms
-  to be translated usually correspond to some concrete notation.\<close>
+  In other words, syntax transformations that operate on input terms written
+  as prefix applications are difficult to make robust. Luckily, this case
+  rarely occurs in practice, because syntax forms to be translated usually
+  correspond to some concrete notation.
+\<close>
 
 
 subsection \<open>Raw syntax and translations \label{sec:syn-trans}\<close>
@@ -1101,14 +1048,13 @@ text \<open>
   \end{tabular}
   \<^medskip>
 
-  Unlike mixfix notation for existing formal entities
-  (\secref{sec:notation}), raw syntax declarations provide full access
-  to the priority grammar of the inner syntax, without any sanity
-  checks.  This includes additional syntactic categories (via
-  @{command nonterminal}) and free-form grammar productions (via
-  @{command syntax}).  Additional syntax translations (or macros, via
-  @{command translations}) are required to turn resulting parse trees
-  into proper representations of formal entities again.
+  Unlike mixfix notation for existing formal entities (\secref{sec:notation}),
+  raw syntax declarations provide full access to the priority grammar of the
+  inner syntax, without any sanity checks. This includes additional syntactic
+  categories (via @{command nonterminal}) and free-form grammar productions
+  (via @{command syntax}). Additional syntax translations (or macros, via
+  @{command translations}) are required to turn resulting parse trees into
+  proper representations of formal entities again.
 
   @{rail \<open>
     @@{command nonterminal} (@{syntax name} + @'and')
@@ -1126,193 +1072,177 @@ text \<open>
     transpat: ('(' @{syntax nameref} ')')? @{syntax string}
   \<close>}
 
-  \<^descr> @{command "nonterminal"}~\<open>c\<close> declares a type
-  constructor \<open>c\<close> (without arguments) to act as purely syntactic
-  type: a nonterminal symbol of the inner syntax.
+  \<^descr> @{command "nonterminal"}~\<open>c\<close> declares a type constructor \<open>c\<close> (without
+  arguments) to act as purely syntactic type: a nonterminal symbol of the
+  inner syntax.
 
-  \<^descr> @{command "syntax"}~\<open>(mode) c :: \<sigma> (mx)\<close> augments the
-  priority grammar and the pretty printer table for the given print
-  mode (default \<^verbatim>\<open>""\<close>). An optional keyword @{keyword_ref
-  "output"} means that only the pretty printer table is affected.
+  \<^descr> @{command "syntax"}~\<open>(mode) c :: \<sigma> (mx)\<close> augments the priority grammar and
+  the pretty printer table for the given print mode (default \<^verbatim>\<open>""\<close>). An
+  optional keyword @{keyword_ref "output"} means that only the pretty printer
+  table is affected.
 
-  Following \secref{sec:mixfix}, the mixfix annotation \<open>mx =
-  template ps q\<close> together with type \<open>\<sigma> = \<tau>\<^sub>1 \<Rightarrow> \<dots> \<tau>\<^sub>n \<Rightarrow> \<tau>\<close> and
-  specify a grammar production.  The \<open>template\<close> contains
-  delimiter tokens that surround \<open>n\<close> argument positions
-  (\<^verbatim>\<open>_\<close>).  The latter correspond to nonterminal symbols
-  \<open>A\<^sub>i\<close> derived from the argument types \<open>\<tau>\<^sub>i\<close> as
-  follows:
+  Following \secref{sec:mixfix}, the mixfix annotation \<open>mx = template ps q\<close>
+  together with type \<open>\<sigma> = \<tau>\<^sub>1 \<Rightarrow> \<dots> \<tau>\<^sub>n \<Rightarrow> \<tau>\<close> and specify a grammar production.
+  The \<open>template\<close> contains delimiter tokens that surround \<open>n\<close> argument
+  positions (\<^verbatim>\<open>_\<close>). The latter correspond to nonterminal symbols \<open>A\<^sub>i\<close> derived
+  from the argument types \<open>\<tau>\<^sub>i\<close> as follows:
 
     \<^item> \<open>prop\<close> if \<open>\<tau>\<^sub>i = prop\<close>
 
-    \<^item> \<open>logic\<close> if \<open>\<tau>\<^sub>i = (\<dots>)\<kappa>\<close> for logical type
-    constructor \<open>\<kappa> \<noteq> prop\<close>
+    \<^item> \<open>logic\<close> if \<open>\<tau>\<^sub>i = (\<dots>)\<kappa>\<close> for logical type constructor \<open>\<kappa> \<noteq> prop\<close>
 
     \<^item> \<open>any\<close> if \<open>\<tau>\<^sub>i = \<alpha>\<close> for type variables
 
-    \<^item> \<open>\<kappa>\<close> if \<open>\<tau>\<^sub>i = \<kappa>\<close> for nonterminal \<open>\<kappa>\<close>
-    (syntactic type constructor)
+    \<^item> \<open>\<kappa>\<close> if \<open>\<tau>\<^sub>i = \<kappa>\<close> for nonterminal \<open>\<kappa>\<close> (syntactic type constructor)
 
-  Each \<open>A\<^sub>i\<close> is decorated by priority \<open>p\<^sub>i\<close> from the
-  given list \<open>ps\<close>; missing priorities default to 0.
+  Each \<open>A\<^sub>i\<close> is decorated by priority \<open>p\<^sub>i\<close> from the given list \<open>ps\<close>; missing
+  priorities default to 0.
 
-  The resulting nonterminal of the production is determined similarly
-  from type \<open>\<tau>\<close>, with priority \<open>q\<close> and default 1000.
-
-  \<^medskip>
-  Parsing via this production produces parse trees \<open>t\<^sub>1, \<dots>, t\<^sub>n\<close> for the argument slots.  The resulting parse tree is
-  composed as \<open>c t\<^sub>1 \<dots> t\<^sub>n\<close>, by using the syntax constant \<open>c\<close> of the syntax declaration.
-
-  Such syntactic constants are invented on the spot, without formal
-  check wrt.\ existing declarations.  It is conventional to use plain
-  identifiers prefixed by a single underscore (e.g.\ \<open>_foobar\<close>).  Names should be chosen with care, to avoid clashes
-  with other syntax declarations.
+  The resulting nonterminal of the production is determined similarly from
+  type \<open>\<tau>\<close>, with priority \<open>q\<close> and default 1000.
 
   \<^medskip>
-  The special case of copy production is specified by \<open>c =\<close>~\<^verbatim>\<open>""\<close> (empty string).
-  It means that the resulting parse tree \<open>t\<close> is copied directly, without any
-  further decoration.
+  Parsing via this production produces parse trees \<open>t\<^sub>1, \<dots>, t\<^sub>n\<close> for the
+  argument slots. The resulting parse tree is composed as \<open>c t\<^sub>1 \<dots> t\<^sub>n\<close>, by
+  using the syntax constant \<open>c\<close> of the syntax declaration.
 
-  \<^descr> @{command "no_syntax"}~\<open>(mode) decls\<close> removes grammar
-  declarations (and translations) resulting from \<open>decls\<close>, which
-  are interpreted in the same manner as for @{command "syntax"} above.
+  Such syntactic constants are invented on the spot, without formal check
+  wrt.\ existing declarations. It is conventional to use plain identifiers
+  prefixed by a single underscore (e.g.\ \<open>_foobar\<close>). Names should be chosen
+  with care, to avoid clashes with other syntax declarations.
 
-  \<^descr> @{command "translations"}~\<open>rules\<close> specifies syntactic
-  translation rules (i.e.\ macros) as first-order rewrite rules on
-  ASTs (\secref{sec:ast}).  The theory context maintains two
-  independent lists translation rules: parse rules (\<^verbatim>\<open>=>\<close>
-  or \<open>\<rightharpoonup>\<close>) and print rules (\<^verbatim>\<open><=\<close> or \<open>\<leftharpoondown>\<close>).
-  For convenience, both can be specified simultaneously as parse~/
-  print rules (\<^verbatim>\<open>==\<close> or \<open>\<rightleftharpoons>\<close>).
+  \<^medskip>
+  The special case of copy production is specified by \<open>c =\<close>~\<^verbatim>\<open>""\<close> (empty
+  string). It means that the resulting parse tree \<open>t\<close> is copied directly,
+  without any further decoration.
 
-  Translation patterns may be prefixed by the syntactic category to be
-  used for parsing; the default is \<open>logic\<close> which means that
-  regular term syntax is used.  Both sides of the syntax translation
-  rule undergo parsing and parse AST translations
-  \secref{sec:tr-funs}, in order to perform some fundamental
-  normalization like \<open>\<lambda>x y. b \<leadsto> \<lambda>x. \<lambda>y. b\<close>, but other AST
-  translation rules are \<^emph>\<open>not\<close> applied recursively here.
+  \<^descr> @{command "no_syntax"}~\<open>(mode) decls\<close> removes grammar declarations (and
+  translations) resulting from \<open>decls\<close>, which are interpreted in the same
+  manner as for @{command "syntax"} above.
 
-  When processing AST patterns, the inner syntax lexer runs in a
-  different mode that allows identifiers to start with underscore.
-  This accommodates the usual naming convention for auxiliary syntax
-  constants --- those that do not have a logical counter part --- by
-  allowing to specify arbitrary AST applications within the term
-  syntax, independently of the corresponding concrete syntax.
+  \<^descr> @{command "translations"}~\<open>rules\<close> specifies syntactic translation rules
+  (i.e.\ macros) as first-order rewrite rules on ASTs (\secref{sec:ast}). The
+  theory context maintains two independent lists translation rules: parse
+  rules (\<^verbatim>\<open>=>\<close> or \<open>\<rightharpoonup>\<close>) and print rules (\<^verbatim>\<open><=\<close> or \<open>\<leftharpoondown>\<close>). For convenience, both
+  can be specified simultaneously as parse~/ print rules (\<^verbatim>\<open>==\<close> or \<open>\<rightleftharpoons>\<close>).
+
+  Translation patterns may be prefixed by the syntactic category to be used
+  for parsing; the default is \<open>logic\<close> which means that regular term syntax is
+  used. Both sides of the syntax translation rule undergo parsing and parse
+  AST translations \secref{sec:tr-funs}, in order to perform some fundamental
+  normalization like \<open>\<lambda>x y. b \<leadsto> \<lambda>x. \<lambda>y. b\<close>, but other AST translation rules
+  are \<^emph>\<open>not\<close> applied recursively here.
+
+  When processing AST patterns, the inner syntax lexer runs in a different
+  mode that allows identifiers to start with underscore. This accommodates the
+  usual naming convention for auxiliary syntax constants --- those that do not
+  have a logical counter part --- by allowing to specify arbitrary AST
+  applications within the term syntax, independently of the corresponding
+  concrete syntax.
 
   Atomic ASTs are distinguished as @{ML Ast.Constant} versus @{ML
-  Ast.Variable} as follows: a qualified name or syntax constant
-  declared via @{command syntax}, or parse tree head of concrete
-  notation becomes @{ML Ast.Constant}, anything else @{ML
-  Ast.Variable}.  Note that \<open>CONST\<close> and \<open>XCONST\<close> within
-  the term language (\secref{sec:pure-grammar}) allow to enforce
-  treatment as constants.
+  Ast.Variable} as follows: a qualified name or syntax constant declared via
+  @{command syntax}, or parse tree head of concrete notation becomes @{ML
+  Ast.Constant}, anything else @{ML Ast.Variable}. Note that \<open>CONST\<close> and
+  \<open>XCONST\<close> within the term language (\secref{sec:pure-grammar}) allow to
+  enforce treatment as constants.
 
-  AST rewrite rules \<open>(lhs, rhs)\<close> need to obey the following
-  side-conditions:
+  AST rewrite rules \<open>(lhs, rhs)\<close> need to obey the following side-conditions:
 
-    \<^item> Rules must be left linear: \<open>lhs\<close> must not contain
-    repeated variables.\<^footnote>\<open>The deeper reason for this is that AST
-    equality is not well-defined: different occurrences of the ``same''
-    AST could be decorated differently by accidental type-constraints or
-    source position information, for example.\<close>
+    \<^item> Rules must be left linear: \<open>lhs\<close> must not contain repeated
+    variables.\<^footnote>\<open>The deeper reason for this is that AST equality is not
+    well-defined: different occurrences of the ``same'' AST could be decorated
+    differently by accidental type-constraints or source position information,
+    for example.\<close>
 
     \<^item> Every variable in \<open>rhs\<close> must also occur in \<open>lhs\<close>.
 
-  \<^descr> @{command "no_translations"}~\<open>rules\<close> removes syntactic
-  translation rules, which are interpreted in the same manner as for
-  @{command "translations"} above.
+  \<^descr> @{command "no_translations"}~\<open>rules\<close> removes syntactic translation rules,
+  which are interpreted in the same manner as for @{command "translations"}
+  above.
 
-  \<^descr> @{attribute syntax_ast_trace} and @{attribute
-  syntax_ast_stats} control diagnostic output in the AST normalization
-  process, when translation rules are applied to concrete input or
-  output.
+  \<^descr> @{attribute syntax_ast_trace} and @{attribute syntax_ast_stats} control
+  diagnostic output in the AST normalization process, when translation rules
+  are applied to concrete input or output.
 
 
-  Raw syntax and translations provides a slightly more low-level
-  access to the grammar and the form of resulting parse trees.  It is
-  often possible to avoid this untyped macro mechanism, and use
-  type-safe @{command abbreviation} or @{command notation} instead.
-  Some important situations where @{command syntax} and @{command
-  translations} are really need are as follows:
+  Raw syntax and translations provides a slightly more low-level access to the
+  grammar and the form of resulting parse trees. It is often possible to avoid
+  this untyped macro mechanism, and use type-safe @{command abbreviation} or
+  @{command notation} instead. Some important situations where @{command
+  syntax} and @{command translations} are really need are as follows:
 
-  \<^item> Iterated replacement via recursive @{command translations}.
-  For example, consider list enumeration @{term "[a, b, c, d]"} as
+  \<^item> Iterated replacement via recursive @{command translations}. For example,
+  consider list enumeration @{term "[a, b, c, d]"} as defined in theory
+  @{theory List} in Isabelle/HOL.
+
+  \<^item> Change of binding status of variables: anything beyond the built-in
+  @{keyword "binder"} mixfix annotation requires explicit syntax translations.
+  For example, consider list filter comprehension @{term "[x \<leftarrow> xs . P]"} as
   defined in theory @{theory List} in Isabelle/HOL.
-
-  \<^item> Change of binding status of variables: anything beyond the
-  built-in @{keyword "binder"} mixfix annotation requires explicit
-  syntax translations.  For example, consider list filter
-  comprehension @{term "[x \<leftarrow> xs . P]"} as defined in theory @{theory
-  List} in Isabelle/HOL.
 \<close>
 
 
 subsubsection \<open>Applying translation rules\<close>
 
-text \<open>As a term is being parsed or printed, an AST is generated as
-  an intermediate form according to \figref{fig:parse-print}.  The AST
-  is normalized by applying translation rules in the manner of a
-  first-order term rewriting system.  We first examine how a single
-  rule is applied.
+text \<open>
+  As a term is being parsed or printed, an AST is generated as an intermediate
+  form according to \figref{fig:parse-print}. The AST is normalized by
+  applying translation rules in the manner of a first-order term rewriting
+  system. We first examine how a single rule is applied.
 
-  Let \<open>t\<close> be the abstract syntax tree to be normalized and
-  \<open>(lhs, rhs)\<close> some translation rule.  A subtree \<open>u\<close>
-  of \<open>t\<close> is called \<^emph>\<open>redex\<close> if it is an instance of \<open>lhs\<close>; in this case the pattern \<open>lhs\<close> is said to match the
-  object \<open>u\<close>.  A redex matched by \<open>lhs\<close> may be
-  replaced by the corresponding instance of \<open>rhs\<close>, thus
-  \<^emph>\<open>rewriting\<close> the AST \<open>t\<close>.  Matching requires some notion
-  of \<^emph>\<open>place-holders\<close> in rule patterns: @{ML Ast.Variable} serves
-  this purpose.
+  Let \<open>t\<close> be the abstract syntax tree to be normalized and \<open>(lhs, rhs)\<close> some
+  translation rule. A subtree \<open>u\<close> of \<open>t\<close> is called \<^emph>\<open>redex\<close> if it is an
+  instance of \<open>lhs\<close>; in this case the pattern \<open>lhs\<close> is said to match the
+  object \<open>u\<close>. A redex matched by \<open>lhs\<close> may be replaced by the corresponding
+  instance of \<open>rhs\<close>, thus \<^emph>\<open>rewriting\<close> the AST \<open>t\<close>. Matching requires some
+  notion of \<^emph>\<open>place-holders\<close> in rule patterns: @{ML Ast.Variable} serves this
+  purpose.
 
-  More precisely, the matching of the object \<open>u\<close> against the
-  pattern \<open>lhs\<close> is performed as follows:
+  More precisely, the matching of the object \<open>u\<close> against the pattern \<open>lhs\<close> is
+  performed as follows:
 
-  \<^item> Objects of the form @{ML Ast.Variable}~\<open>x\<close> or @{ML
-  Ast.Constant}~\<open>x\<close> are matched by pattern @{ML
-  Ast.Constant}~\<open>x\<close>.  Thus all atomic ASTs in the object are
-  treated as (potential) constants, and a successful match makes them
-  actual constants even before name space resolution (see also
-  \secref{sec:ast}).
+    \<^item> Objects of the form @{ML Ast.Variable}~\<open>x\<close> or @{ML Ast.Constant}~\<open>x\<close> are
+    matched by pattern @{ML Ast.Constant}~\<open>x\<close>. Thus all atomic ASTs in the
+    object are treated as (potential) constants, and a successful match makes
+    them actual constants even before name space resolution (see also
+    \secref{sec:ast}).
 
-  \<^item> Object \<open>u\<close> is matched by pattern @{ML
-  Ast.Variable}~\<open>x\<close>, binding \<open>x\<close> to \<open>u\<close>.
+    \<^item> Object \<open>u\<close> is matched by pattern @{ML Ast.Variable}~\<open>x\<close>, binding \<open>x\<close> to
+    \<open>u\<close>.
 
-  \<^item> Object @{ML Ast.Appl}~\<open>us\<close> is matched by @{ML
-  Ast.Appl}~\<open>ts\<close> if \<open>us\<close> and \<open>ts\<close> have the
-  same length and each corresponding subtree matches.
+    \<^item> Object @{ML Ast.Appl}~\<open>us\<close> is matched by @{ML Ast.Appl}~\<open>ts\<close> if \<open>us\<close> and
+    \<open>ts\<close> have the same length and each corresponding subtree matches.
 
-  \<^item> In every other case, matching fails.
+    \<^item> In every other case, matching fails.
 
+  A successful match yields a substitution that is applied to \<open>rhs\<close>,
+  generating the instance that replaces \<open>u\<close>.
 
-  A successful match yields a substitution that is applied to \<open>rhs\<close>, generating the instance that replaces \<open>u\<close>.
+  Normalizing an AST involves repeatedly applying translation rules until none
+  are applicable. This works yoyo-like: top-down, bottom-up, top-down, etc. At
+  each subtree position, rules are chosen in order of appearance in the theory
+  definitions.
 
-  Normalizing an AST involves repeatedly applying translation rules
-  until none are applicable.  This works yoyo-like: top-down,
-  bottom-up, top-down, etc.  At each subtree position, rules are
-  chosen in order of appearance in the theory definitions.
-
-  The configuration options @{attribute syntax_ast_trace} and
-  @{attribute syntax_ast_stats} might help to understand this process
-  and diagnose problems.
+  The configuration options @{attribute syntax_ast_trace} and @{attribute
+  syntax_ast_stats} might help to understand this process and diagnose
+  problems.
 
   \begin{warn}
-  If syntax translation rules work incorrectly, the output of
-  @{command_ref print_syntax} with its \<^emph>\<open>rules\<close> sections reveals the
-  actual internal forms of AST pattern, without potentially confusing
-  concrete syntax.  Recall that AST constants appear as quoted strings
-  and variables without quotes.
+  If syntax translation rules work incorrectly, the output of @{command_ref
+  print_syntax} with its \<^emph>\<open>rules\<close> sections reveals the actual internal forms
+  of AST pattern, without potentially confusing concrete syntax. Recall that
+  AST constants appear as quoted strings and variables without quotes.
   \end{warn}
 
   \begin{warn}
-  If @{attribute_ref eta_contract} is set to \<open>true\<close>, terms
-  will be \<open>\<eta>\<close>-contracted \<^emph>\<open>before\<close> the AST rewriter sees
-  them.  Thus some abstraction nodes needed for print rules to match
-  may vanish.  For example, \<open>Ball A (\<lambda>x. P x)\<close> would contract
-  to \<open>Ball A P\<close> and the standard print rule would fail to
-  apply.  This problem can be avoided by hand-written ML translation
-  functions (see also \secref{sec:tr-funs}), which is in fact the same
-  mechanism used in built-in @{keyword "binder"} declarations.
+  If @{attribute_ref eta_contract} is set to \<open>true\<close>, terms will be
+  \<open>\<eta>\<close>-contracted \<^emph>\<open>before\<close> the AST rewriter sees them. Thus some abstraction
+  nodes needed for print rules to match may vanish. For example, \<open>Ball A (\<lambda>x.
+  P x)\<close> would contract to \<open>Ball A P\<close> and the standard print rule would fail to
+  apply. This problem can be avoided by hand-written ML translation functions
+  (see also \secref{sec:tr-funs}), which is in fact the same mechanism used in
+  built-in @{keyword "binder"} declarations.
   \end{warn}
 \<close>
 
@@ -1347,10 +1277,9 @@ text \<open>
    @@{ML_antiquotation syntax_const}) name
   \<close>}
 
-  \<^descr> @{command parse_translation} etc. declare syntax translation
-  functions to the theory.  Any of these commands have a single
-  @{syntax text} argument that refers to an ML expression of
-  appropriate type as follows:
+  \<^descr> @{command parse_translation} etc. declare syntax translation functions to
+  the theory. Any of these commands have a single @{syntax text} argument that
+  refers to an ML expression of appropriate type as follows:
 
   \<^medskip>
   {\footnotesize
@@ -1368,110 +1297,108 @@ text \<open>
   \end{tabular}}
   \<^medskip>
 
-  The argument list consists of \<open>(c, tr)\<close> pairs, where \<open>c\<close> is the syntax name of the formal entity involved, and \<open>tr\<close> a function that translates a syntax form \<open>c args\<close> into
-  \<open>tr ctxt args\<close> (depending on the context).  The Isabelle/ML
-  naming convention for parse translations is \<open>c_tr\<close> and for
-  print translations \<open>c_tr'\<close>.
+  The argument list consists of \<open>(c, tr)\<close> pairs, where \<open>c\<close> is the syntax name
+  of the formal entity involved, and \<open>tr\<close> a function that translates a syntax
+  form \<open>c args\<close> into \<open>tr ctxt args\<close> (depending on the context). The
+  Isabelle/ML naming convention for parse translations is \<open>c_tr\<close> and for print
+  translations \<open>c_tr'\<close>.
 
   The @{command_ref print_syntax} command displays the sets of names
-  associated with the translation functions of a theory under \<open>parse_ast_translation\<close> etc.
+  associated with the translation functions of a theory under
+  \<open>parse_ast_translation\<close> etc.
 
-  \<^descr> \<open>@{class_syntax c}\<close>, \<open>@{type_syntax c}\<close>,
-  \<open>@{const_syntax c}\<close> inline the authentic syntax name of the
-  given formal entities into the ML source.  This is the
-  fully-qualified logical name prefixed by a special marker to
-  indicate its kind: thus different logical name spaces are properly
-  distinguished within parse trees.
+  \<^descr> \<open>@{class_syntax c}\<close>, \<open>@{type_syntax c}\<close>, \<open>@{const_syntax c}\<close> inline the
+  authentic syntax name of the given formal entities into the ML source. This
+  is the fully-qualified logical name prefixed by a special marker to indicate
+  its kind: thus different logical name spaces are properly distinguished
+  within parse trees.
 
-  \<^descr> \<open>@{const_syntax c}\<close> inlines the name \<open>c\<close> of
-  the given syntax constant, having checked that it has been declared
-  via some @{command syntax} commands within the theory context.  Note
-  that the usual naming convention makes syntax constants start with
-  underscore, to reduce the chance of accidental clashes with other
-  names occurring in parse trees (unqualified constants etc.).
+  \<^descr> \<open>@{const_syntax c}\<close> inlines the name \<open>c\<close> of the given syntax constant,
+  having checked that it has been declared via some @{command syntax} commands
+  within the theory context. Note that the usual naming convention makes
+  syntax constants start with underscore, to reduce the chance of accidental
+  clashes with other names occurring in parse trees (unqualified constants
+  etc.).
 \<close>
 
 
 subsubsection \<open>The translation strategy\<close>
 
-text \<open>The different kinds of translation functions are invoked during
-  the transformations between parse trees, ASTs and syntactic terms
-  (cf.\ \figref{fig:parse-print}).  Whenever a combination of the form
-  \<open>c x\<^sub>1 \<dots> x\<^sub>n\<close> is encountered, and a translation function
-  \<open>f\<close> of appropriate kind is declared for \<open>c\<close>, the
-  result is produced by evaluation of \<open>f [x\<^sub>1, \<dots>, x\<^sub>n]\<close> in ML.
+text \<open>
+  The different kinds of translation functions are invoked during the
+  transformations between parse trees, ASTs and syntactic terms (cf.\
+  \figref{fig:parse-print}). Whenever a combination of the form \<open>c x\<^sub>1 \<dots> x\<^sub>n\<close>
+  is encountered, and a translation function \<open>f\<close> of appropriate kind is
+  declared for \<open>c\<close>, the result is produced by evaluation of \<open>f [x\<^sub>1, \<dots>, x\<^sub>n]\<close>
+  in ML.
 
-  For AST translations, the arguments \<open>x\<^sub>1, \<dots>, x\<^sub>n\<close> are ASTs.  A
-  combination has the form @{ML "Ast.Constant"}~\<open>c\<close> or @{ML
-  "Ast.Appl"}~\<open>[\<close>@{ML Ast.Constant}~\<open>c, x\<^sub>1, \<dots>, x\<^sub>n]\<close>.
-  For term translations, the arguments are terms and a combination has
-  the form @{ML Const}~\<open>(c, \<tau>)\<close> or @{ML Const}~\<open>(c, \<tau>)
-  $ x\<^sub>1 $ \<dots> $ x\<^sub>n\<close>.  Terms allow more sophisticated transformations
-  than ASTs do, typically involving abstractions and bound
-  variables. \<^emph>\<open>Typed\<close> print translations may even peek at the type
-  \<open>\<tau>\<close> of the constant they are invoked on, although some
-  information might have been suppressed for term output already.
+  For AST translations, the arguments \<open>x\<^sub>1, \<dots>, x\<^sub>n\<close> are ASTs. A combination
+  has the form @{ML "Ast.Constant"}~\<open>c\<close> or @{ML "Ast.Appl"}~\<open>[\<close>@{ML
+  Ast.Constant}~\<open>c, x\<^sub>1, \<dots>, x\<^sub>n]\<close>. For term translations, the arguments are
+  terms and a combination has the form @{ML Const}~\<open>(c, \<tau>)\<close> or @{ML
+  Const}~\<open>(c, \<tau>) $ x\<^sub>1 $ \<dots> $ x\<^sub>n\<close>. Terms allow more sophisticated
+  transformations than ASTs do, typically involving abstractions and bound
+  variables. \<^emph>\<open>Typed\<close> print translations may even peek at the type \<open>\<tau>\<close> of the
+  constant they are invoked on, although some information might have been
+  suppressed for term output already.
 
-  Regardless of whether they act on ASTs or terms, translation
-  functions called during the parsing process differ from those for
-  printing in their overall behaviour:
+  Regardless of whether they act on ASTs or terms, translation functions
+  called during the parsing process differ from those for printing in their
+  overall behaviour:
 
-  \<^descr>[Parse translations] are applied bottom-up.  The arguments are
-  already in translated form.  The translations must not fail;
-  exceptions trigger an error message.  There may be at most one
-  function associated with any syntactic name.
+    \<^descr>[Parse translations] are applied bottom-up. The arguments are already in
+    translated form. The translations must not fail; exceptions trigger an
+    error message. There may be at most one function associated with any
+    syntactic name.
 
-  \<^descr>[Print translations] are applied top-down.  They are supplied
-  with arguments that are partly still in internal form.  The result
-  again undergoes translation; therefore a print translation should
-  not introduce as head the very constant that invoked it.  The
-  function may raise exception @{ML Match} to indicate failure; in
-  this event it has no effect.  Multiple functions associated with
-  some syntactic name are tried in the order of declaration in the
-  theory.
+    \<^descr>[Print translations] are applied top-down. They are supplied with
+    arguments that are partly still in internal form. The result again
+    undergoes translation; therefore a print translation should not introduce
+    as head the very constant that invoked it. The function may raise
+    exception @{ML Match} to indicate failure; in this event it has no effect.
+    Multiple functions associated with some syntactic name are tried in the
+    order of declaration in the theory.
 
-
-  Only constant atoms --- constructor @{ML Ast.Constant} for ASTs and
-  @{ML Const} for terms --- can invoke translation functions.  This
-  means that parse translations can only be associated with parse tree
-  heads of concrete syntax, or syntactic constants introduced via
-  other translations.  For plain identifiers within the term language,
-  the status of constant versus variable is not yet know during
-  parsing.  This is in contrast to print translations, where constants
-  are explicitly known from the given term in its fully internal form.
+  Only constant atoms --- constructor @{ML Ast.Constant} for ASTs and @{ML
+  Const} for terms --- can invoke translation functions. This means that parse
+  translations can only be associated with parse tree heads of concrete
+  syntax, or syntactic constants introduced via other translations. For plain
+  identifiers within the term language, the status of constant versus variable
+  is not yet know during parsing. This is in contrast to print translations,
+  where constants are explicitly known from the given term in its fully
+  internal form.
 \<close>
 
 
 subsection \<open>Built-in syntax transformations\<close>
 
 text \<open>
-  Here are some further details of the main syntax transformation
-  phases of \figref{fig:parse-print}.
+  Here are some further details of the main syntax transformation phases of
+  \figref{fig:parse-print}.
 \<close>
 
 
 subsubsection \<open>Transforming parse trees to ASTs\<close>
 
-text \<open>The parse tree is the raw output of the parser.  It is
-  transformed into an AST according to some basic scheme that may be
-  augmented by AST translation functions as explained in
-  \secref{sec:tr-funs}.
+text \<open>
+  The parse tree is the raw output of the parser. It is transformed into an
+  AST according to some basic scheme that may be augmented by AST translation
+  functions as explained in \secref{sec:tr-funs}.
 
   The parse tree is constructed by nesting the right-hand sides of the
-  productions used to recognize the input.  Such parse trees are
-  simply lists of tokens and constituent parse trees, the latter
-  representing the nonterminals of the productions.  Ignoring AST
-  translation functions, parse trees are transformed to ASTs by
-  stripping out delimiters and copy productions, while retaining some
-  source position information from input tokens.
+  productions used to recognize the input. Such parse trees are simply lists
+  of tokens and constituent parse trees, the latter representing the
+  nonterminals of the productions. Ignoring AST translation functions, parse
+  trees are transformed to ASTs by stripping out delimiters and copy
+  productions, while retaining some source position information from input
+  tokens.
 
-  The Pure syntax provides predefined AST translations to make the
-  basic \<open>\<lambda>\<close>-term structure more apparent within the
-  (first-order) AST representation, and thus facilitate the use of
-  @{command translations} (see also \secref{sec:syn-trans}).  This
-  covers ordinary term application, type application, nested
-  abstraction, iterated meta implications and function types.  The
-  effect is illustrated on some representative input strings is as
+  The Pure syntax provides predefined AST translations to make the basic
+  \<open>\<lambda>\<close>-term structure more apparent within the (first-order) AST
+  representation, and thus facilitate the use of @{command translations} (see
+  also \secref{sec:syn-trans}). This covers ordinary term application, type
+  application, nested abstraction, iterated meta implications and function
+  types. The effect is illustrated on some representative input strings is as
   follows:
 
   \begin{center}
@@ -1489,85 +1416,83 @@ text \<open>The parse tree is the raw output of the parser.  It is
   \end{center}
 
   Note that type and sort constraints may occur in further places ---
-  translations need to be ready to cope with them.  The built-in
-  syntax transformation from parse trees to ASTs insert additional
-  constraints that represent source positions.
+  translations need to be ready to cope with them. The built-in syntax
+  transformation from parse trees to ASTs insert additional constraints that
+  represent source positions.
 \<close>
 
 
 subsubsection \<open>Transforming ASTs to terms\<close>
 
-text \<open>After application of macros (\secref{sec:syn-trans}), the AST
-  is transformed into a term.  This term still lacks proper type
-  information, but it might contain some constraints consisting of
-  applications with head \<^verbatim>\<open>_constrain\<close>, where the second
-  argument is a type encoded as a pre-term within the syntax.  Type
-  inference later introduces correct types, or indicates type errors
-  in the input.
+text \<open>
+  After application of macros (\secref{sec:syn-trans}), the AST is transformed
+  into a term. This term still lacks proper type information, but it might
+  contain some constraints consisting of applications with head \<^verbatim>\<open>_constrain\<close>,
+  where the second argument is a type encoded as a pre-term within the syntax.
+  Type inference later introduces correct types, or indicates type errors in
+  the input.
 
-  Ignoring parse translations, ASTs are transformed to terms by
-  mapping AST constants to term constants, AST variables to term
-  variables or constants (according to the name space), and AST
-  applications to iterated term applications.
+  Ignoring parse translations, ASTs are transformed to terms by mapping AST
+  constants to term constants, AST variables to term variables or constants
+  (according to the name space), and AST applications to iterated term
+  applications.
 
-  The outcome is still a first-order term.  Proper abstractions and
-  bound variables are introduced by parse translations associated with
-  certain syntax constants.  Thus \<^verbatim>\<open>("_abs" x x)\<close> eventually
-  becomes a de-Bruijn term \<^verbatim>\<open>Abs ("x", _, Bound 0)\<close>.
+  The outcome is still a first-order term. Proper abstractions and bound
+  variables are introduced by parse translations associated with certain
+  syntax constants. Thus \<^verbatim>\<open>("_abs" x x)\<close> eventually becomes a de-Bruijn term
+  \<^verbatim>\<open>Abs ("x", _, Bound 0)\<close>.
 \<close>
 
 
 subsubsection \<open>Printing of terms\<close>
 
-text \<open>The output phase is essentially the inverse of the input
-  phase.  Terms are translated via abstract syntax trees into
-  pretty-printed text.
+text \<open>
+  The output phase is essentially the inverse of the input phase. Terms are
+  translated via abstract syntax trees into pretty-printed text.
 
   Ignoring print translations, the transformation maps term constants,
   variables and applications to the corresponding constructs on ASTs.
-  Abstractions are mapped to applications of the special constant
-  \<^verbatim>\<open>_abs\<close> as seen before.  Type constraints are represented
-  via special \<^verbatim>\<open>_constrain\<close> forms, according to various
-  policies of type annotation determined elsewhere.  Sort constraints
-  of type variables are handled in a similar fashion.
+  Abstractions are mapped to applications of the special constant \<^verbatim>\<open>_abs\<close> as
+  seen before. Type constraints are represented via special \<^verbatim>\<open>_constrain\<close>
+  forms, according to various policies of type annotation determined
+  elsewhere. Sort constraints of type variables are handled in a similar
+  fashion.
 
-  After application of macros (\secref{sec:syn-trans}), the AST is
-  finally pretty-printed.  The built-in print AST translations reverse
-  the corresponding parse AST translations.
+  After application of macros (\secref{sec:syn-trans}), the AST is finally
+  pretty-printed. The built-in print AST translations reverse the
+  corresponding parse AST translations.
 
   \<^medskip>
   For the actual printing process, the priority grammar
-  (\secref{sec:priority-grammar}) plays a vital role: productions are
-  used as templates for pretty printing, with argument slots stemming
-  from nonterminals, and syntactic sugar stemming from literal tokens.
+  (\secref{sec:priority-grammar}) plays a vital role: productions are used as
+  templates for pretty printing, with argument slots stemming from
+  nonterminals, and syntactic sugar stemming from literal tokens.
 
-  Each AST application with constant head \<open>c\<close> and arguments
-  \<open>t\<^sub>1\<close>, \dots, \<open>t\<^sub>n\<close> (for \<open>n = 0\<close> the AST is
-  just the constant \<open>c\<close> itself) is printed according to the
-  first grammar production of result name \<open>c\<close>.  The required
-  syntax priority of the argument slot is given by its nonterminal
-  \<open>A\<^sup>(\<^sup>p\<^sup>)\<close>.  The argument \<open>t\<^sub>i\<close> that corresponds to the
-  position of \<open>A\<^sup>(\<^sup>p\<^sup>)\<close> is printed recursively, and then put in
-  parentheses \<^emph>\<open>if\<close> its priority \<open>p\<close> requires this.  The
-  resulting output is concatenated with the syntactic sugar according
-  to the grammar production.
+  Each AST application with constant head \<open>c\<close> and arguments \<open>t\<^sub>1\<close>, \dots,
+  \<open>t\<^sub>n\<close> (for \<open>n = 0\<close> the AST is just the constant \<open>c\<close> itself) is printed
+  according to the first grammar production of result name \<open>c\<close>. The required
+  syntax priority of the argument slot is given by its nonterminal \<open>A\<^sup>(\<^sup>p\<^sup>)\<close>.
+  The argument \<open>t\<^sub>i\<close> that corresponds to the position of \<open>A\<^sup>(\<^sup>p\<^sup>)\<close> is printed
+  recursively, and then put in parentheses \<^emph>\<open>if\<close> its priority \<open>p\<close> requires
+  this. The resulting output is concatenated with the syntactic sugar
+  according to the grammar production.
 
-  If an AST application \<open>(c x\<^sub>1 \<dots> x\<^sub>m)\<close> has more arguments than
-  the corresponding production, it is first split into \<open>((c x\<^sub>1
-  \<dots> x\<^sub>n) x\<^sub>n\<^sub>+\<^sub>1 \<dots> x\<^sub>m)\<close> and then printed recursively as above.
+  If an AST application \<open>(c x\<^sub>1 \<dots> x\<^sub>m)\<close> has more arguments than the
+  corresponding production, it is first split into \<open>((c x\<^sub>1 \<dots> x\<^sub>n) x\<^sub>n\<^sub>+\<^sub>1 \<dots>
+  x\<^sub>m)\<close> and then printed recursively as above.
 
-  Applications with too few arguments or with non-constant head or
-  without a corresponding production are printed in prefix-form like
-  \<open>f t\<^sub>1 \<dots> t\<^sub>n\<close> for terms.
+  Applications with too few arguments or with non-constant head or without a
+  corresponding production are printed in prefix-form like \<open>f t\<^sub>1 \<dots> t\<^sub>n\<close> for
+  terms.
 
-  Multiple productions associated with some name \<open>c\<close> are tried
-  in order of appearance within the grammar.  An occurrence of some
-  AST variable \<open>x\<close> is printed as \<open>x\<close> outright.
+  Multiple productions associated with some name \<open>c\<close> are tried in order of
+  appearance within the grammar. An occurrence of some AST variable \<open>x\<close> is
+  printed as \<open>x\<close> outright.
 
   \<^medskip>
-  White space is \<^emph>\<open>not\<close> inserted automatically.  If
-  blanks (or breaks) are required to separate tokens, they need to be
-  specified in the mixfix declaration (\secref{sec:mixfix}).
+  White space is \<^emph>\<open>not\<close> inserted automatically. If blanks (or breaks) are
+  required to separate tokens, they need to be specified in the mixfix
+  declaration (\secref{sec:mixfix}).
 \<close>
 
 end
